---
title: Abstract Algebra by Pinter, Chapter 19
author: Amir Taaki
header-includes: |
    - \usepackage{mathrsfs}
    - \usepackage{mathtools}
    - \usepackage{extpfeil}
    - \DeclareMathOperator\ker{ker}
    - \DeclareMathOperator\ord{ord}
    - \DeclareMathOperator\gcd{gcd}
    - \DeclareMathOperator\lcm{lcm}
    - \DeclareMathOperator\mod{mod}
abstract: Chapter 19 on Quotient Rings
---

# A. Examples of Quotient Rings

## Q1

$$A = \mathbb{Z}_{10}, J = \{ 0, 5 \}$$

\begin{align*}
J = J + 0 &= \{ 0, 5 \} \\
J + 1 &= \{ 1, 6 \} \\
J + 2 &= \{ 2, 7 \} \\
J + 3 &= \{ 3, 8 \} \\
J + 4 &= \{ 4, 9 \}
\end{align*}

\begin{tabular}{c | c c c c c c c c c}
    $+$ & J   & J + 1 & J + 2 & J + 3 & J + 4 \\
    \cline{1-6}
J     &   J   & J + 1 & J + 2 & J + 3 & J + 4 \\
J + 1 & J + 1 & J + 2 & J + 3 & J + 4 & J     \\
J + 2 & J + 2 & J + 3 & J + 4 & J     & J + 1 \\
J + 3 & J + 3 & J + 4 & J     & J + 1 & J + 2 \\
J + 4 & J + 4 & J     & J + 1 & J + 2 & J + 3 \\
\end{tabular}

\begin{tabular}{c | c c c c c c c c c}
$\cdot$ & J   & J + 1 & J + 2 & J + 3 & J + 4 \\
    \cline{1-6}
J     &   J   & J     & J     & J     & J     \\
J + 1 & J     & J + 1 & J + 2 & J + 3 & J + 4 \\
J + 2 & J     & J + 2 & J + 4 & J + 1 & J + 3 \\
J + 3 & J     & J + 3 & J + 1 & J + 4 & J + 2 \\
J + 4 & J     & J + 4 & J + 3 & J + 2 & J + 1 \\
\end{tabular}

## Q2

$$A = P_3, J = \{ \varnothing, \{a\}\}$$

\begin{align*}
J = J + 0 &= \{ \varnothing, \{a \}\} \\
J + \{ b \} &= \{ \{b\}, \{a, b \}\} \\
J + \{ c \} &= \{ \{c\}, \{a, c \}\} \\
J + \{ b, c \} &= \{ \{b, c\}, \{a, b, c \}\} \\
\end{align*}

\begin{tabular}{c | c c c c c c c c c}
    $+$ &       J         & J + \{b\}   & J + \{c\}   & J + \{b,c\} \\
    \cline{1-5}    
J           &   J         & J + \{b\}   & J + \{c\}   & J + \{b,c\} \\
J + \{b\}   & J + \{b\}   & J           & J + \{b,c\} & J + \{c\}   \\
J + \{c\}   & J + \{c\}   & J + \{b,c\} & J           & J + \{b\}   \\
J + \{b,c\} & J + \{b,c\} & J + \{c\}   & J + \{b\}   & J           \\
\end{tabular}

\begin{tabular}{c | c c c c c c c c c}
$\cdot$ &       J         & J + \{b\}   & J + \{c\}   & J + \{b,c\} \\
    \cline{1-5}    
J           & J           & J           & J           & J           \\
J + \{b\}   & J           & J + \{b\}   & J           & J + \{b\}   \\
J + \{c\}   & J           & J           & J + \{c\}   & J + \{c\}   \\
J + \{b,c\} & J           & J + \{b\}   & J + \{c\}   & J + \{b,c\} \\
\end{tabular}

## Q3

$$A = \mathbb{Z}_2 \times \mathbb{Z}_6, J = \{(0, 0), (0, 2), (0, 4)\}$$

\begin{align*}
J &= \{(0, 0), (0, 2), (0, 4)\} \\
J + (0, 1) &= \{(0, 1), (0, 3), (0, 5)\} \\
J + (1, 0) &= \{(1, 0), (1, 2), (1, 4)\} \\
J + (1, 1) &= \{(1, 1), (1, 3), (1, 5)\} \\
\end{align*}

\begin{tabular}{c | c c c c c c c c c}
    $+$ &       J         & J + (0,1)   & J + (1,0)   & J + (1,1)   \\
    \cline{1-5}    
J           &   J         & J + (0,1)   & J + (1,0)   & J + (1,1)   \\
J + (0,1)   & J + (0,1)   & J           & J + (1,1)   & J + (1,0)   \\
J + (1,0)   & J + (1,0)   & J + (1,1)   & J           & J + (0,1)   \\
J + (1,1)   & J + (1,1)   & J + (1,0)   & J + (0,1)   & J           \\
\end{tabular}

\begin{tabular}{c | c c c c c c c c c}
$\cdot$ &       J         & J + (0,1)   & J + (1,0)   & J + (1,1)   \\
    \cline{1-5}    
J           &   J         & J           & J           & J           \\
J + (0,1)   & J           & J + (0,1)   & J           & J + (0,1)   \\
J + (1,0)   & J           & J           & J + (1,0)   & J + (1,0)   \\
J + (1,1)   & J           & J + (0,1)   & J + (1,0)   & J + (1,1)   \\
\end{tabular}

# B. Examples of the Use of the FHT

## Q1

$$f(x) = x \mod 5$$
$$\ker f = \{ 0, 5, 10, 15 \} = \langle 5 \rangle$$
$$\mathbb{Z}_5 \cong \mathbb{Z}_{20} / \langle 5 \rangle$$

\begin{align*}
J = J + 0 &= \{ 0, 5, 10, 15 \} \\
J + 1 &= \{ 1, 6, 11, 16 \} \\
J + 2 &= \{ 2, 7, 12, 17 \} \\
J + 3 &= \{ 3, 8, 13, 18 \} \\
J + 4 &= \{ 4, 9, 14, 19 \}
\end{align*}

\begin{tabular}{c | c c c c c c c c c}
    $+$ & J   & J + 1 & J + 2 & J + 3 & J + 4 \\
    \cline{1-6}
J     &   J   & J + 1 & J + 2 & J + 3 & J + 4 \\
J + 1 & J + 1 & J + 2 & J + 3 & J + 4 & J     \\
J + 2 & J + 2 & J + 3 & J + 4 & J     & J + 1 \\
J + 3 & J + 3 & J + 4 & J     & J + 1 & J + 2 \\
J + 4 & J + 4 & J     & J + 1 & J + 2 & J + 3 \\
\end{tabular}

\begin{tabular}{c | c c c c c c c c c}
$\cdot$ & J   & J + 1 & J + 2 & J + 3 & J + 4 \\
    \cline{1-6}
J     &   J   & J     & J     & J     & J     \\
J + 1 & J     & J + 1 & J + 2 & J + 3 & J + 4 \\
J + 2 & J     & J + 2 & J + 4 & J + 1 & J + 3 \\
J + 3 & J     & J + 3 & J + 1 & J + 4 & J + 2 \\
J + 4 & J     & J + 4 & J + 3 & J + 2 & J + 1 \\
\end{tabular}

Tables are exact same for mod 5.

## Q2

$$f(x) = x \mod 3$$
$$\ker f = \{ 0, 3 \} = \langle 3 \rangle$$
$$\mathbb{Z}_3 \cong \mathbb{Z}_6 / \langle 3 \rangle$$

\begin{align*}
J = J + 0 &= \{ 0, 3 \} \\
J + 1 &= \{ 1, 4 \} \\
J + 2 &= \{ 2, 5 \} \\
\end{align*}

\begin{tabular}{c | c c c c c c c c c}
    $+$ & J   & J + 1 & J + 2 \\
    \cline{1-4}
J     &   J   & J + 1 & J + 2 \\
J + 1 & J + 1 & J + 2 & J  \\
J + 2 & J + 2 & J     & J + 1 \\
\end{tabular}

\begin{tabular}{c | c c c c c c c c c}
$\cdot$ & J   & J + 1 & J + 2 \\
    \cline{1-4}
J     &   J   & J     & J     \\
J + 1 & J     & J + 1 & J + 2 \\
J + 2 & J     & J + 2 & J + 1 \\
\end{tabular}

Tables are exact same for mod 3.

## Q3

$$P_2 = \{ \varnothing, \{a\}, \{b\}, \{a, b\}\}$$
$$P_3 = \{ \varnothing, \{a\}, \{b\}, \{c\}, \{a,b\}, \{a,c\}, \{b,c\}, \{a,b,c\} \}$$
\begin{align*}
K = K + \varnothing &= \{ \varnothing, \{ c \} \} \\
K + \{ a \} &= \{ \{ a \}, \{ a, c \} \} \\
K + \{ b \} &= \{ \{ b \}, \{ b, c \} \} \\
K + \{ a, b \} &= \{ \{ a, b \}, \{ a, b, c \} \} \\
\end{align*}
$$f(X) = X \cap \{ a, b \}$$
$$f : P_3 \rightarrow P_2$$
$$P_2 \cong P_3 / \langle \{ \varnothing, \{ c \} \} \rangle$$

\begin{tabular}{c | c c c c c c c c c}
    $+$     & K           & K + \{a\}   & K + \{b\}   & K + \{a,b\} \\
    \cline{1-5}
K           &   K         & K + \{a\}   & K + \{b\}   & K + \{a,b\} \\
K + \{a\}   & K + \{a\}   & K           & K + \{a,b\} & K + \{b\}   \\
K + \{b\}   & K + \{b\}   & K + \{a,b\} & K           & K + \{a\}   \\
K + \{a,b\} & K + \{a,b\} & K + \{b\}   & K + \{a\}   & K           \\
\end{tabular}

\begin{tabular}{c | c c c c c c c c c}
$\cdot$     & K           & K + \{a\}   & K + \{b\}   & K + \{a,b\} \\
    \cline{1-5}
K           & K           & K           & K           & K           \\
K + \{a\}   & K           & K + \{a\}   & K           & K + \{a\}   \\
K + \{b\}   & K           & K           & K + \{b\}   & K + \{b\}   \\
K + \{a,b\} & K           & K + \{a\}   & K + \{b\}   & K + \{a,b\} \\
\end{tabular}

## Q4

$$f: \mathbb{Z}_2 \times \mathbb{Z}_2 \rightarrow \mathbb{Z}_2$$
$$f((x, y)) = x$$
$$K = \{ (0,0), (0, 1) \}$$
$$K + (1, 0) = \{ (1,0), (1,1) \}$$

\begin{tabular}{c | c c c c c c c c c}
    $+$     & K           & K + (1,0) \\
    \cline{1-3}                
K           &   K         & K + (1,0) \\
K + (1,0)   & K + (1,0)   & K         \\
\end{tabular}

\begin{tabular}{c | c c c c c c c c c}
$\cdot$     & K           & K + (1,0) \\
    \cline{1-3}                
K           &   K         & K         \\
K + (1,0)   & K           & K + (1,0) \\
\end{tabular}

# C. Quotient Rings and Homomorphic Images in $\mathcal{F}(\mathbb{R})$

## Q1

$$\phi : \mathcal{F}(\mathbb{R}) \rightarrow \mathbb{R} \times \mathbb{R}$$
$$\phi(f) = (f(0), f(1))$$

1. $\phi(f + g) = ((f + g)(0), (f + g)(1)) = (f(0), f(1)) + (g(0), g(1)) = \phi(f) + \phi(g)$
2. $\phi(f \cdot g) = ((f \cdot g)(0), (f \cdot g)(1)) = (f(0), f(1))(g(0), g(1)) = \phi(f)\phi(g)$

Let $f(x) = (a - b)x + b$, then $f \in \mathcal{F}(\mathbb{R})$, $f(0) = b$ and $f(1) = a$. Thus functions of this form can represent any value in $\mathbb{R} \times \mathbb{R}$ and so the homomorphism $\phi$ is *onto* $\mathbb{R} \times \mathbb{R}$.

$$K = \{ f \in \mathcal{F}(\mathbb{R}) : f(0) = 0 \text{ and } f(1) = 0 \}$$

## Q2

$$J = \{ f \in \mathcal{F}(\mathbb{R}) : f(0) = 0 \text{ and } f(1) = 0 \}$$

Thus $J$ is the kernel of the homomorphism $\phi$. The kernel is also an ideal of $\mathcal{F}(\mathbb{R})$, so
$$\mathcal{F}(\mathbb{R}) / J \cong \mathbb{R} \times \mathbb{R}$$

## Q3

$$\phi: \mathcal{F}(\mathbb{R}) \rightarrow \mathcal{F}(\mathbb{Q}, \mathbb{R})$$
$$\phi(f) = f_{\mathbb{Q}} = \text{ the restriction of } f \text{ to } \mathbb{Q}$$

$\phi$ is onto because $\forall g \in \mathcal{F}(\mathbb{Q}, \mathbb{R}), \exists f \in \mathcal{F}(\mathbb{R}) : g = f_{\mathbb{Q}}$. $\phi$ is a homomorphism since $\phi(f \cdot g) = \phi(f) \cdot \phi(g)$ and $\phi(f + g) = \phi(f) + \phi(g)$.

$$K = \{ f \in \mathcal{F}(\mathbb{R}) : f(x) = 0 \}$$

## Q4

$J$ is also the kernel of $\mathcal{F}(\mathbb{R})$, which means it is also an ideal. Thus
$$\mathcal{F}(\mathbb{R}) / J \cong \mathcal{F}(\mathbb{Q})$$

# D. Elementary Applications of the Fundamental Homomorphism Theorem

## Q1

Note that ring is commutative then
$$(x + y)^2 = x(x + y) + y(x + y) = x^2 + xy + yx + y^2 = x^2 + 2xy + y^2 = x^2 + y^2$$

So $h(x) = x^2$ is a homomorphism since $h(x + y) = x^2 + y^2 = h(x) + h(y)$ and $h(xy) = x^2 y^2 = h(x) h(y)$

$$J = \{x \in A : x^2 = 0 \}$$
$$B = \{ x^2 : x \in A \}$$

$h$ is a homomorphism from $A$ to $B$ and the kernel is $J$
$$A/J \cong B$$

## Q2

$h(x) = 3x$ is a homomorphism because $h(x + y) = 3x + 3y = h(x) + h(y)$ and $h(xy) = h(x) h(y)$ because
$$h(xy) = 3xy = 6xy + 3xy = (3x)(3y) = h(x)h(y)$$

$J = \{ x : 3x = 0 \}$ is the kernel and thus ideal of $h$. $B = \{ 3x : x \in A \}$ is a subring of $A$ by the homomorphism shown above
$$A/J \cong B$$

## Q3

$$\pi_a(xy) = axy = a^2 xy = (ax)(ay) = \pi_a(x)\pi_a(y)$$
$$\pi_a(x + y) = a(x + y) = ax + ay = \pi_a(x) + \pi_a(y)$$
$$I_a = \{ x \in A : ax = 0 \} = \ker \pi_a$$
$$\pi_a(1) = a$$
$$\pi_a(x) = \pi_a(x \cdot 1) = a + \cdots + a \in \langle a \rangle$$
$$\pi_a : A \rightarrow \langle a \rangle$$
$$A / I_a \cong \langle a \rangle$$

## Q4

$$\phi(ab) = \pi_{ab} = \pi_a \pi_b = \phi(a) \phi(b)$$
$$\phi(a + b) = \pi_{a + b} = \pi_a + \pi_b = \phi(a) + \phi(b)$$
$$I = \{ x \in A : ax = 0, \forall a \in A \}$$
$$\pi_a(x) = ax$$
$$\bar{A} = \{ \pi_a : a \in A \}$$
$$\phi(a) = \pi_a$$
$$\ker \phi = \{ x \in A : \phi(x) = \pi_0 \}$$
$$\forall a \in A \qquad \pi_0(a) = 0$$
$$\therefore \ker \phi = I$$
$$\phi : A \rightarrow \bar{A}$$
$$A/I \cong \bar{A}$$

# E. Properties of Quotient Rings $A/J$ in Relation to Properties of $J$

## Q1

*Every element of $A/J$ has a square root iff for every $x \in A$, there is some $y \in A$ such that $x - y^2 \in J$.*

Let $J + x \in A/J$ then
$$J + x = (J + y)(J + y)$$
But $J$ is ideal and so absorbs products in $A$
$$J + x = J + y^2$$
$$J + x - y^2 = J$$
$$x - y^2 \in J$$

## Q2

*Every element of $A/J$ is its own negative iff $x + x \in J$ for every $x \in A$.*

$$\forall x \in A, x + x \in J \implies J + x + x = J$$
$$\therefore \forall x \in A \qquad J + x = -(J + x)$$

## Q3

*$A/J$ is a boolean ring iff $x^2 - x \in J$ for every $x \in A$.*

$$(J + x)^2 - (J + x) = J^2 + Jx + xJ + x^2 - J - x$$
But noting J absorbs products
$$(J+x)^2 - (J + x) = J + x^2 - x$$
But $x^2 - x \in J$ so
$$J + x^2 - x = J$$
so $A/J$ is a boolean ring.

## Q4

*If $J$ is the ideal of all the nilpotent elements of commutative ring $A$, then $A/J$ has no nilpotent elements (except zero).*

$$a \in J \implies a^n = 0 \text{ for some } n$$
Let $x \in A : x \notin J \implies x^n \neq 0$
$$(J + x)^n = J + x^n \neq J$$
Thus $\forall x \in A : x \in J$, $J + x$ is not nilpotent.

## Q5

*Every element of $A/J$ is nilpotent iff $J$ has the following property: for every $x \in A$, there is a positive integer $n$ such that $x^n \in J$.*

$$\forall x \in A, x^n \in J$$
$$(J + x)^n = J + x^n = J$$
Thus every element of $A/J$ is nilpotent.

## Q6

*$A/J$ has a unity element iff there exists an element $a \in A$ such that $ax - x \in J$ and $xa - x \in J$ for every $x \in A$.*

\begin{align*}
(J + a)(J + x) &= J + x \\
               &= J + ax \\
(J + x)(J + a) &= J + x \\
               &= J + xa
\end{align*}

$$J + x = J + ax$$
$$J + ax - x = J$$
So $ax - x \in J$
Likewise
$$J + xa = J + x$$
$$J + xa - x = J$$
$$\implies xa - x \in J$$

# F. Prime and Maximal Ideals

Let $A$ be a commutative ring with unity, and $J$ an ideal of $A$. Prove the following:

## Q1

*$A/J$ is a commutative ring with unity.*

$$(J + x)(J + y) = J + xy$$
But $xy = yx$
$$J + xy = J + yx$$
$$\implies (J + x)(J + y) = (J + y)(J + x)$$

$$(J + 1_A)(J + x) = J + x$$

## Q2

*$J$ is a prime ideal iff $A/J$ is an integral domain.*

Assume $J$ is a prime ideal.

$$ab \in J \implies a \in J \text{ or } b \in J$$
$$J + ab = J + ac \implies J + b = J + c$$
Let $J + ab = J + ac$
$$J + ab - ac = J$$
$$a(b - c) \in J$$

But $a \notin J, b \notin J$ and $c \notin J$
$$\implies b - c \in J$$
$$J + b = J + c$$

Thus
$$J + ab = J + ac \implies J + b = J + c$$

For the converse, assume $a \notin J$, if $a \in J$, then we are done, otherwise
$$J + ab = J + a0 \implies J + b = J + 0$$
$$J + ab = J \implies J + b = J$$
$$a(b - c) \in J \implies b - c \in J$$
$$ab \in J \implies b \in J$$

## Q3

*Every maximal ideal of $A$ is a prime ideal.*

Let $J$ be a maximal ideal of $A$.

Then $A/J$ is a field.

Every field is an integral domain, so $A/J$ is an integral domain.

Since $A/J$ is an integral domain, so $J$ is a prime ideal.

## Q4

*If $A/J$ is a field, then $J$ is a maximal ideal.*

$$\phi(x) = J + x$$
$$j \in J, \phi(j) = J$$
$A/J$ is a field, so ideal is $J$, which is maximal.

# G. Further Properties of Quotient Rings in Relation to Their Ideals

## Q1

*Prove that $A/J$ is a field iff for every element $a \in A$, where $a \notin J$, there is some $b \in A$ such that $ab - 1 \in J.$*

$$(J + a)(J + b) = J + ab = J + 1 \implies ab - 1 \in J$$

## Q2

*Prove that every nonzero element of $A/J$ is either invertible or a divisor of zero iff the following property holds, where $a, x \in A$: For every $a \notin J$, there is some $x \notin J$ such that either $ax \in J$ or $ax - 1 \in J$.*

$$ax - 1 \in J \implies (J + a)(J + x) = J + 1$$
and thus $J + a$ is invertible.

$$ax \in J \implies (J + a)(J + x) = J$$
and so $J + a$ is a divisor of zero.

## Q3

*An ideal $J$ of a ring $A$ is called primary iff for all $a, b \in A$, if $ab \in J$, then either $a \in J$ or $b^n \in J$ for some positive integer $n$. Prove that every zero divisor in $A/J$ is nilpotent iff $J$ is primary.*

Nilpotent means $(J + x)^n = J$, but $(J + x)^n = J + x^n$, that is $x^n \in J$. Every zero divisor in $A/J$ means $(J + a)(J + b) = J + ab = J$ or that $ab \in J$. Thus either $a^1 \in J$ or $b^n \in J$. Thus we can say that $J + b$ is nilpotent since $(J + b)^n = J$.

## Q4

*An ideal $J$ of a ring $A$ is called semiprime iff it has the following property: For every $a \in A$, if $a^n \in J$ for some positive integer $n$, then necessarily $a \in J$. Prove that $J$ is semiprime iff $A/J$ has no nilpotent elements (except zero).*

$A/J$ has no nilpotent elements means that $J + x^n \neq J$ for any integer $n$. Thus for every $a \in A: a \notin J$, then $a^n \notin J$. If $A/J$ has a nilpotent element, then $J$ cannot be semiprime because $a \notin J$ and $a^n \in J$ is a contradiction. This also holds true in reverse since $a^n \in J$ where $a \notin J$ would imply $J$ is not semiprime.

## Q5

*Prove that an integral domain can have no nonzero nilpotent elements. Then use part 4, together with Exercise F2, to prove that every prime ideal in a commutative ring is semiprime.*

Nilpotent elements are also zero divisors since $a^n = 0 = a \cdot a^{n - 1}$. So an integral domain cannot have nilpotent elements.

From F2, we learn that if $J$ is a prime ideal, then $A/J$ is an integral domain (no nilpotent elements). From the last exercise, we see that if $A/J$ has no nilpotent elements, then $J$ is semiprime.

# H. $\mathbb{Z}_n$ as a Homomorphic Image of $\mathbb{Z}$

## Q1

$$x^2 - 7y^2 - 24 = 0$$
$$\phi : \mathbb{Z} \rightarrow \mathbb{Z}_7$$
$$x^2 - 3 = 0$$
$$x^2 = 3$$
$$\forall x \in \mathbb{Z}_7, x^2 \neq 3$$
No solution.

## Q2

$$x^2 + (x + 1)^2 + (x + 2)^2 = y^2$$
$$3x^2 + 6x + 5 = y^2$$
$$\phi : \mathbb{Z} \rightarrow \mathbb{Z}_3$$
$$y^2 = 2$$
$$\forall y \in \mathbb{Z}_3, y^2 \neq 2$$
No solution.

## Q3

$$x^2 + 10y^2 = 10n + a, a \in \{ 2, 3, 7, 8 \}$$
$$\phi : \mathbb{Z} \rightarrow \mathbb{Z}_{10}$$
$$x^2 = a$$
\begin{align*}
0^2 &= 0 \\
1^2 &= 1 \\
2^2 &= 4 \\
3^2 &= 9 \\
4^2 &= 6 \\
5^2 &= 5 \\
6^2 &= 6 \\
7^2 &= 9 \\
8^2 &= 6 \\
9^2 &= 1 \\
\end{align*}
No solution.

## Q4

$$3, 8, 13, 18, 23, \dots = \langle 3 \rangle$$
$$x \in \mathbb{Z}_5 : x^2 = 3$$
\begin{align*}
0^2 &= 0 \\
1^2 &= 1 \\
2^2 &= 4 \\
3^2 &= 4 \\
4^2 &= 1 \\
\end{align*}

## Q5

$$2, 10, 18, 26, \dots = \langle 2 \rangle$$
$$x \in \mathbb{Z}_8 : x^3 = 2$$
\begin{align*}
0^3 &= 0 \\
1^3 &= 1 \\
2^3 &= 0 \\
3^3 &= 1 \\
4^3 &= 0 \\
5^3 &= 5 \\
6^3 &= 0 \\
7^3 &= 7 \\
\end{align*}

## Q6

$$3, 11, 19, 27, \dots = \langle 3 \rangle$$
$$x \in \mathbb{Z}_8 : x^2 + y^2 = 3$$
\begin{align*}
0^2 &= 0 \\
1^2 &= 1 \\
2^2 &= 4 \\
3^2 &= 1 \\
4^2 &= 0 \\
5^2 &= 1 \\
6^2 &= 4 \\
7^2 &= 1 \\
\end{align*}
For any $a \in \mathbb{Z}_8, a^2 = 1$ or $a^2 = 4$, so $\nexists x, y \in \mathbb{Z}_8 : x^2 + y^2 = 3$

## Q7

$$n(n + 1) = 10u + a, a \in \{ 0, 2, 6 \}$$
$$\phi : \mathbb{Z} \rightarrow \mathbb{Z}_{10}$$
\begin{align*}
0 \cdot 1 &= 0 \\
1 \cdot 2 &= 2 \\
2 \cdot 3 &= 6 \\
3 \cdot 4 &= 2 \\
4 \cdot 5 &= 0 \\
5 \cdot 6 &= 0 \\
6 \cdot 7 &= 2 \\
7 \cdot 8 &= 6 \\
8 \cdot 9 &= 2 \\
9 \cdot 0 &= 0 \\
\end{align*}
Thus $n(n + 1) \in \{ 0, 2, 6 \}$

## Q8

$$n(n + 1)(n + 2) = 10u + a, a \in \{ 0, 4, 6 \}$$
$$\phi : \mathbb{Z} \rightarrow \mathbb{Z}_{10}$$
\begin{align*}
0 \cdot 1 \cdot 2 &= 0 \\
1 \cdot 2 \cdot 3 &= 6 \\
2 \cdot 3 \cdot 4 &= 4 \\
3 \cdot 4 \cdot 5 &= 0 \\
4 \cdot 5 \cdot 6 &= 0 \\
5 \cdot 6 \cdot 7 &= 0 \\
6 \cdot 7 \cdot 8 &= 6 \\
7 \cdot 8 \cdot 9 &= 4 \\
8 \cdot 9 \cdot 0 &= 0 \\
9 \cdot 0 \cdot 1 &= 0 \\
\end{align*}

