---
title: Abstract Algebra by Pinter, Chapter 22
author: Amir Taaki
header-includes: |
    - \usepackage{mathrsfs}
    - \usepackage{mathtools}
    - \usepackage{extpfeil}
    - \DeclareMathOperator\ker{ker}
    - \DeclareMathOperator\ord{ord}
    - \DeclareMathOperator\gcd{gcd}
    - \DeclareMathOperator\lcm{lcm}
    - \DeclareMathOperator\mod{mod}
    - \DeclareMathOperator\char{char}
    - \DeclareMathOperator\max{max}
abstract: Chapter 22 on Factoring Into Primes
---

# A. Properties of the Relation "$a$" divides "$b$"

## Q1

*If $a|b$ and $b|c$, then $a|c$.*

$$a|b \implies b = ka$$
$$b|c \implies c = lb$$

$$c = l(ka) = (kl)a \implies a|c$$

## Q2

*$a|b$ iff $a|(-b)$ iff $(-a)|b$.*

$$b = ka \iff -b = (-k)a \iff b = (-k)(-a)$$
$$a|b \iff a|(-b) \iff (-a)|b$$

## Q3

*$1|a$ and $(-1)|a$.*

$a = 1 \cdot a = (-1) \cdot (-a)$ thus $1|a$ and $(-1)|a$

## Q4

*$a|0$.*

$$0 = 0a \therefore a|0$$

## Q5

*If $c|a$ and $c|b$, then $c|(ax + by)$ for all $x, y \in \mathbb{Z}$.*

$c|a$ and $c|b \implies a = kc$ and $b = lc$

$$ax + by = kcx + lcy = c(kx + ly)$$
$$\implies c|(ax + by)$$

## Q6

*If $a > 0$ and $b > 0$ and $a|b$, then $a \leq b$.*

Let $b = ka$

$k \neq 0$ because $0a = 0 = b$ but $b > 0$

If $k < 0$ then $-k > 0$ or $-k \geq 1 \implies 1 \leq -ka = -b$ which is a contradiction since $b > 0$.

Thus $k > 0$

$$0 < k$$
$$1 \leq k$$
$$a \leq ka = b$$

## Q7

*$a|b$ iff $ac|bc$, when $c \neq 0$.*

$bc = kac \implies b = ka$ by the cancellation property.

## Q8

*If $a|b$ and $c|d$, then $ac|bd$.*

$$b = ka \qquad d = lc$$

$$bd = (ka)(lc) = (kl)ac$$

## Q9

*Let $p$ be a prime. If $p|a^n$ for some $n > 0$, then $p|a$.*

$$a^n = (p_1 \cdots p_r)(p_1 \cdots p_r)(p_1 \cdots p_r)$$

$$p | a^n \implies a^n = kp$$

Since $a^n$ factors uniquely $\implies p | a$

# B. Properties of the gcd

Prove the following, for any integers $a, b$, and $c$. For each of these problems, you will need only the
definition of the gcd.

## Q1

*If $a > 0$ and $a|b$, then $\gcd(a, b) = a$.*

$$b = ka$$

Let $t = \gcd(a, b)$ then
\begin{align*}
t &= ax + by \\
&= ax + (ka)y \\
&= a(x + ky)
\end{align*}

$$\gcd(a, b) = a$$

$a$ is the gcd because it is the biggest divisor in $a$.

## Q2

*$gcd(a, 0) = a$, if $a > 0$.*

$$a|a \text{ and } a|0 \implies \gcd(a, 0) = a$$

## Q3

*$\gcd(a, b) = \gcd(a, b + xa)$ for any $x \in \mathbb{Z}$ .*

Let $t = \gcd(a, b)$

$$t = ka + lb$$

$$a = wu \qquad b + xa = vu \text{ from } \gcd(a, b + xa)$$

$$b + xa = b + x(wu) = vu$$
$$b = u(v - xw)$$

but

\begin{align*}
t &= ka + lb \\
&= k(wu) + lu(v - xw) \\
&= u(kw + l(v - xw))
\end{align*}

therefore it follows $u|t$

Since $\gcd(a, b + xa) = \bar{k}a + \bar{l}(b + xa) = \bar{k}(tr) + \bar{l}(ts + x(tr))$

Therefore $t$ is also the $\gcd$ of $a$ and $bx + a$.

$$\gcd(a, b) = \gcd(a, b + xa) \qquad \forall x \in \mathbb{Z}$$

## Q4

*Let $p$ be a prime. Then $\gcd(a, p) = 1$ or $p$. (Explain.)*

$a$ is a composite of primes.

That is $a = p_1 \cdots p_r$

If $a = pk$ for some $k$, then

1. $p|p$ and $p|a$.
2. for any integer $u$, since $p$ is prime, $u$ does not divide $p$.

Thus according to the definition $\gcd(a, p) = p$

Otherwise $\gcd(a, p) = 1$ because $p$ is indivisible and does not divide $a$.

## Q5

*Suppose every common divisor of $a$ and $b$ is a common divisor of $c$ and $d$, and vice versa. Then $\gcd(a, b) = \gcd(c, d)$.*

$$\gcd(a, b) > \gcd(c, d)$$

$$\implies p_1 \cdots p_i p_j \cdots p_r > p_1 \cdots p_i$$

where $p_1 \cdots p_i$ are the prime common factors of $\gcd(a, b)$ and $\gcd(c, d)$ or $\gcd(\gcd(a, b), \gcd(c, d))$.

Then this implies that $a$ and $b$ have common factors $p_j \cdots p_r$ which are not in $c$ and $d$.

Hence $\gcd(a, b) = \gcd(c, d)$.

## Q6

*If $\gcd(ab, c) = 1$, then $gcd(a, c) = 1$ and $gcd(b, c) = 1$.*

Let $ab = (p_1 \cdots p_r)(q_1 \cdots q_s)$

$$\gcd(ab, c) = 1 \implies \forall p_i, q_j \qquad p_i \not| c, q_j \not|c$$

$$\forall p_i \not| c \implies \gcd(a, c) = 1$$

Likewise for $b$.

## Q7

*Let $\gcd(a, b) = c$. Write $a = ca'$ and $b = cb'$. Then $\gcd(a', b') = 1$.*

Let $\gcd(a', b') = x$

$$a = ca' = ckx$$
$$b = cb' = clx$$
$$\gcd(a, b) = cx$$

but $\gcd(a, b) = c \implies x = 1$
$$\therefore \gcd(a', b') = 1$$

# C. Properties of Relatively Prime Integers

## Q1

From theorem 3,
$$\gcd(a, b) = ra + sb \text{ for some integers } r \text{ and } s$$
But $a \perp b$, so $\gcd(a, b) = 1$. That is,
$$ra + sb = 1$$

## Q2

$$\gcd(a, c) = 1 \implies a \perp c \implies a \nmid c$$
But $c \mid ab$ so $ab = ch$ for some integer $h$.
And $\gcd(a, c) = 1$
$$\implies ka + lc = 1$$
$$\implies kab + lcb = b$$
However $ab = ch$, so
$$kch + lcb = b$$
$$c(kh + lb) = b$$
Thus $c \mid b$

## Q3

$$d = pa = qc$$
$$\gcd(a, c) = 1 \implies ka + lc = 1$$
$$kad + lcd = d$$
$$ka(qc) + lc(pa) = d$$
$$ac(kq + lp) = d$$
$$ac \mid d$$

## Q4

$$ka + lc = 1$$
$$kab + lcb = b$$
$$k(pd) + l(qd) = b$$
$$d(kp + lq) = b$$
$$d \mid b$$

## Q5

$$d = ka + lb$$
$$a = dr \qquad b = ds$$
\begin{align*}
d &= kdr + lds \\
&= d(kr + ls)
\end{align*}
$$kr + ls = 1 \implies \gcd(r, s) = 1$$

## Q6

$$ka + lc = 1$$
$$hb + jc = 1$$

$$ka(hb + jc) + lc = 1$$
$$kh(ab) + (j + l)c = 1 \implies gcd(ab, c) = 1$$

# D. Further Properties of gcd's and Relatively Prime Integers

## Q1

$$b = ma = nc$$
$$ka + lc = d$$
$$b(ka + lc) = bd$$
$$bka + blc = bd$$
$$(nc)ka + (ma)lc = bd$$
$$nk \cdot ac + ml \cdot ac = bd$$
$$\implies ac \mid bd$$

## Q2

$$b = mac = nad$$
$$kc + ld = 1$$
$$bkc + bld = b$$
$$(nad)kc + (mac)ld = b$$
$$acd(nk + ml) = b$$

## Q3

From theorem 3,
$$J = \{ ua + vb : u, v \in \mathbb{Z} \}$$
$J$ is a principal ideal of $\mathbb{Z}$ and $J = \langle d \rangle$.

Since $x \in J$, then $x$ is a multiple of $d$ and so $d \mid x$.

Likewise $d \mid x \implies x \in J$ and so $x$ is a linear combination of $a$ and $b$.

## Q4

Let $J$ be a linear combination of $a$ and $b$.

$t = \gcd(a, b)$ and $J = \langle t \rangle$

Thus $t = ka + lb$ but $x \mid a$ and $x \mid b$ so $x \mid t$.

But $t \mid c$, so $c \in J$ and so $c$ is a multiple of $t$ (which is the biggest divisor of $a$ and $b$).

$$t \leq c$$

$c \mid c \implies c \mid a$ and $c \mid b$, and $c$ is the greatest divisor of $c$. So $c = \gcd(a, b) = t$.

See also [here](https://math.stackexchange.com/questions/2627981/suppose-that-for-all-integers-x-xa-and-xb-if-and-only-if-xc-then-c)

## Q5

$$\forall n > 0, \text{ if } \gcd(a, b) = 1 \text{ then } \gcd(a, b^n) = 1$$

$\gcd(a, b) = 1$ means there is only the shared divisor of $1$ between $a$ and $b$.

That there is no $u > 1$ such that $a = xu$ and $b = yu$.

Assume $\gcd(a, b^k) = 1$, then there is no common divisor between $a$ and $b^k$ and also $a$ and $b$. This means that $a$ and $b^{k + 1}$ also share no prime factors, hence
$$\gcd(a, b^{k + 1}) = 1$$

## Q6

*Suppose $\gcd(a, b) = 1$ and $c|ab$. Then there exist integers $r$ and $s$ such that $c = rs, r|a, s|b$, and $\gcd(r, s) = 1$.*

\begin{align*}
a &= p_1 \cdots p_n \\
b &= q_1 \cdots q_m
\end{align*}

Since $\gcd(a, b) = 1$, $a$ and $b$ share no factors as their prime factors are unique and distinct.

$$c \mid ab \implies ab = kc$$

Since $c$ divides $ab$, it consists of some number of factors of $ab$ such that
$$c = (p_1 \cdots p_i)(q_1 \cdots q_j)$$
that divides $ab$.

Let $r = (p_1 \cdots p_i)$ and $s = (q_1 \cdots q_j)$.

Then $c = rs$, $r \mid a$, $s \mid b$ and $\gcd(r, s) = 1$.

# E. A Property of the $\gcd$

## Q1

*Suppose $a$ is odd and $b$ is even, or vice versa. Then $\gcd(a, b) = \gcd(a + b, a - b)$.*

$a + b$ and $a - b$ is odd.

$t$ is a common divisor of $a - b$ and $a + b$. Since they are both odd, then $t$ is odd.

Sum of $a + b$ and $a - b$ is $2a$, and difference is $2b$.

Since $a + b = tx$ and $a - b = ty$, then
$$(a + b) + (a - b) = tx + ty = t(x + y)$$
Likewise
$$(a + b) - (a - b) = t(x - y)$$

Since $t$ is odd, $t \mid 2a \implies t \mid a$, and also $t \mid b$ thus if $t = \gcd(a + b, a - b)$, then
$$\gcd(a, b) = \gcd(a + b, a - b)$$

## Q2

*Suppose $a$ and $b$ are both odd. Then $2\gcd(a, b) = \gcd(a + b, a - b)$.*

$a$ and $b$ are both odd.

$a + b$ and $a - b$ are thus even.

$t$ is a common divisor of $a + b$ and $a - b$. So $t$ is even.

$$(a + b) + (a - b) = 2a = t(x + y)$$
$$(a + b) - (a - b) = 2b = t(x - y)$$

That is $2|t$ and so $t = 2\gcd(a, b)$ but $t = \gcd(a + b, a - b)$
$$2 \gcd(a, b) = \gcd(a + b, a - b)$$

## Q3

*If $a$ and $b$ are both even, explain why either of the two previous conclusions are possible.*

$$a = 2n \qquad b = 2m$$
$$\gcd(a, b) = t = 2x$$
$$a + b = 2(n + m) \qquad a - b = 2(n - m)$$
$$\gcd(a + b, a - b) = s = 2y$$

$$2a = t(x + y) \qquad 2b = t(x - y)$$

$a$ and $b$ are even, so is $t$.

Thus either case is true: $t \mid a$ or $t \mid 2a$.

There isn't enough information to infer whether $t = \gcd(a, b)$ or $t = 2\gcd(a, b)$.

# F. Least Common Multiples

## Q1

*Prove: The set of all the common multiples of $a$ and $b$ is an ideal of $\mathbb{Z}$.*

$$I = \{ n \cdot \lcm(a, b): n \in \mathbb{Z} \}$$

$$x, y \in I, x + y = i \cdot \lcm(a, b) + j \cdot \lcm(a, b) = (i + j) \cdot \lcm(a, b)$$
$$-x = -i \cdot \lcm(a, b) \in I$$

because if $a \mid c$ then $a \mid -c$

Lastly let $w \in \mathbb{Z}$
$$w \cdot x = (wi) \cdot \lcm(a, b)$$
and since $wi \in \mathbb{Z}$, so $w \cdot x \in I$.

So $I$ is an ideal of $\mathbb{Z}$.

## Q2

*Prove: Every pair of integers $a$ and $b$ has a least common multiple.*

Every ideal of $\mathbb{Z}$ is principal.

That means there exists a generator
$$I = \{ n \cdot \lcm(a, b) : n \in \mathbb{Z} \} = \langle t \rangle $$
which is a least value.

By the well ordering principle $t = 1 \cdot \lcm(a, b) = \lcm(a, b)$.

Since $x \mid xy$ for integers $x, y \in \mathbb{Z}$ where $x \neq 0$ and $y \neq 0$, then $I$ must contain $xy$ and is non-trivial.

## Q3

*Prove $a \cdot \lcm(b, c) = \lcm(ab, ac)$.*

$$l = \lcm(ab, ac)$$
then
$$l = abx = acy$$
for some integers $x$ and $y$.

So $a$ is a factor of $l$
$$l = am$$
$$am = abx = acy$$
thus
$$m = \lcm(b, c)$$

$$a \cdot \lcm(b, c) = \lcm(ab, ac)$$

## Q4

*If $a = a_1 c$ and $b = b_1 c$ where $c = \gcd(a, b)$, then $\lcm(a, b) = a_1 b_1 c$.*

$$\lcm(a, b) = \lcm(a_1 c, b_1 c) = c \cdot \lcm(a_1, b_1)$$ 

But $\gcd(a, b) = c$ and $\gcd(a_1 c, b_1 c) = c$ so $\gcd(a_1, b_1) = 1$. Since there is no $q$ such that both $q \mid a_1$ and $q \mid b_1$, then
\begin{align*}
\lcm(a, b) &= ax = by \\
&= a_1 cx = b_1 cy \\
&= cm \\
m &= a_1 x = b_1 y
\end{align*}

We know that $\gcd(a_1, b_1) = 1$, which means $a_1$ and $b_1$ contain unique prime factors. That is that $x = b_1$ and $y = a_1$.

$$\lcm(a, b) = a_1 b_1 c$$

## Q5

*Prove $\lcm(a, ab) = ab$*

\begin{align*}
\lcm(a, ab) &= a \cdot \lcm(1, b) \\
&= ab
\end{align*}

## Q6

*If $\gcd(a, b) = 1$ then $\lcm(a, b) = ab$.*

From 4,
\begin{align*}
a &= a_1 \gcd(a, b)
&= a_1 \cdot 1 = a_1
\end{align*}
and also $b = b_1$, so
\begin{align*}
\lcm(a, b) &= a_1 b_1 c \\
&= ab \cdot \gcd(a, b) \\
&= ab
\end{align*}

## Q7

*If $\lcm(a, b) = ab$ then $\gcd(a, b) = 1$.*

\begin{align*}
\lcm(a_1 c, b_1 c) &= c \cdot \lcm(a_1, b_1) \\
ab &= c \cdot \lcm(a_1, b_1) \\
(a_1 c)(b_1 c) &= c \cdot \lcm(a_1, b_1) \\
a_1 b_1 c &= \lcm(a_1, b_1)
\end{align*}

But $\gcd(a_1, b_1) = 1 \implies \lcm(a_1, b_1) = a_1 b_1$ so
\begin{align*}
a_1 b_1 c &= a_1 b_1 \\
c &= 1 \\
\gcd(a, b) &= 1
\end{align*}

## Q8

*Let $\gcd(a, b) = c$. Then $\lcm(a, b) = ab/c$.*

\begin{align*}
\lcm(a, b) &= \lcm(a_1 c, b_1 c) \\
&= c \cdot \lcm(a_1, b_1)
\end{align*}

but $\gcd(a, b) = \gcd(a_1 c, b_1 c) = c \implies \gcd(a_1, b_1) = 1$ so $\lcm(a_1, b_1) = a_1 b_1$.

\begin{align*}
\lcm(a, b) &= c \cdot \lcm(a_1, b_1) \\
&= c a_1 b_1 \\
&= (a_1 c)(b_1 c) / c \\
&= ab / c
\end{align*}

## Q9

*Let $\gcd(a, b) = c$ and $\lcm(a, b) = d$. Then $cd = ab$.*

$$\lcm(a, b) = d = ab / c$$
$$cd = ab$$

# G. Ideals in $\mathbb{Z}$

## Q1

*$\langle n \rangle$ is a prime ideal iff $n$ is a prime number.*

Prime ideal:

*if $ab \in J$ then $a \in J$ or $b \in J$*.

Let $J = \langle n \rangle$ be a prime ideal in $\mathbb{Z}$.

Then $J = \{ nx : x \in \mathbb{Z} \}$

Let $y \in J$, then $y = nx$ and $n \in J$.

Let $J = \langle n = uv \rangle$ where $n$ is non-prime.

Then $uv \in J$ but $u \notin J$ and $v \notin J$, so $n$ must be prime.

## Q2

*Every prime ideal of is a maximal ideal.*

$\langle p \rangle \subseteq \langle a \rangle$ so $p \in \langle a \rangle$ but $\langle p \rangle \neq \langle a \rangle \implies p \neq a$ and so $p = a \cdot n$ for some $n \in \mathbb{Z}$.

But $p$ is prime and since $\langle p \rangle \subseteq \langle a \rangle$, then $a < p$, but $a \nmid p$ and $\gcd(a, p) = 1$.

$p \in \langle a \rangle \implies p = a \cdot n$ for some $n \in \mathbb{Z}$ but $\gcd(a, p) = 1 \implies n = p$, therefore $a = 1$ and so $\langle a \rangle = \mathbb{Z}$. Thus every prime ideal $\langle p \rangle$ of $\mathbb{Z}$ is a maximal ideal.

## Q3

*For every prime number $p$, $\mathbb{Z}_p$ is a field.*

Prime ideal:

*if $ab \in J$ then $a \in J$ or $b \in J$*.

Definition of a field: a commutative ring with unity where every nonzero element is invertible.

Every field is an integral domain.

Definition of an integral domain: a commutative ring with unity having the cancellation property. That is $ab = ac \implies b = c$.

From the end of chapter 19 on quotient rings, we have $J$ is a maximal ideal of $A$ (proven above).

$A = \mathbb{Z}$ is a commutative ring with unity so the coset $J + 1$ is the unity of $A/J$ since $(J + 1)(J + a) = J + a$.

Now finally to prove $A/J$ is a field we must show for every $a$, there exists $x$ such that
$$(J + a)(J + x) = J + 1$$

$$K = \{ xa + j : x \in A, j \in J \}$$

$K$ is an ideal, $a \in K$ because $a = 1a + 0$ and $\forall j \in J$, $j \in K$ because $j = 0a + j$.

$K$ is an ideal and contains $J$, but also $a \notin J$ and $a \in K$ so $K$ is bigger than $J$.

But $J$ is maximal so $K = A$.

Therefore $1 \in K$ so $1 = xa + j$ for some $x \in A$ and $j \in J$, that is $1 - xa = j \in J$.
$$J + 1 = J + xa = (J + x)(J + a)$$
So $J + x$ is the multiplicative inverse of $J + a$.

Thus $A/J$ is a field.

## Q4

*If $c = \lcm(a, b)$, then $\langle a \rangle \cap \langle b \rangle = \langle c \rangle$.*

$$c = \lcm(a, b)$$

$\langle c \rangle = \{ n \cdot c : n \in \mathbb{Z} \}$ therefore $\langle c \rangle$ contains all the multiples of $a$ and $b$.

$\langle a \rangle$ is all the multiples of $a$, $\langle b \rangle$ contains all the multiples of $b$, and $\langle a \rangle \cap \langle b \rangle$ are all the multiples of $a$ and $b$.

Any $x \in \langle a \rangle \cap \langle b \rangle$ is both in $\langle a \rangle$ and $\langle b \rangle$ and so is a multiple of both $a$ and $b$. Therefore $x \in \langle c \rangle$.

$$\langle a \rangle \cap \langle b \rangle = \langle c \rangle$$

## Q5

Let $\phi$ be a homomorphism such that
$$\phi: \mathbb{Z} \rightarrow A$$
And let $J$ be the ideal of $\phi$.

Every ideal of $\mathbb{Z}$ is principal. By the well ordering principle pick the least value $n \in J$, and let $m$ be any element of $J$. By the division algorithm $m = nq + r$ where $0 \leq r < n$. Since $n \in J$ and $m \in J$, then $r = m - nq \in J$. So either $r = 0$ or $r > 0$. But $n$ is the least value in $J$, so $r = 0$. So $m = nq$.
$$J = \langle n \rangle$$
$$\mathbb{Z}_n = \mathbb{Z} / \langle n \rangle$$
Since the ideal of $\phi$ is $\langle n \rangle$, so
$$A \cong \mathbb{Z} / \langle n \rangle$$
Every homomorphic image of $\mathbb{Z}$ is isomorphic to $\mathbb{Z}_n$ for some $n$.

## Q6

*Let $G$ be a group and let $a, b \in G$. Then $S = \{ n \in \mathbb{Z}: ab^n = b^n a \}$ is an ideal of $\mathbb{Z}$.*

$S$ is an ideal of $\mathbb{Z}$ if it satisfies the following conditions:

1. $(S, +)$ is a subgroup of $(\mathbb{Z}, +)$
2. For every $r \in \mathbb{Z}$ and every $x \in S$, the product $rx$ is in $S$

Prove $S$ is closed under addition for $x, y \in S$:

\begin{align*}
ab^{x + y} &= ab^x b^y = b^x a b^y \\
           &= b^x b^y a \\
           &= b^{x + y} a
\end{align*}

Prove that for any $x \in S$, that $-x \in S$:

\begin{align*}
ab^n &= b^n a \\
b^{-n} ab^n &= a \\
b^{-n} a &= ab^{-n}
\end{align*}

Lastly prove that for any $r \in \mathbb{Z}$ and every $x \in S$, the product $rx \in S$.

Observe firstly that $ab^n = b^n a$ and then note that $ab^{nx} = a\underbrace{b^n b^n \cdots b^n}_{x \text{ times}}$.
But $b^n = a^{-1} b^n a$.

\begin{align*}
ab^{nx} &= a \underbrace{(a^{-1} b^n a)}_{b^n} b^n \cdots b^n \\
&= (b^n a) b^n \cdots b^n \\
&= (b^n a) (a^{-1} b^n a) \cdots b^n \\
&= b^n (b^n a) \cdots b^n \\
&= b^{nx} a
\end{align*}

And so $S$ is an ideal of $\mathbb{Z}$.

## Q7

*Let $G$ be a group, $H$ a subgroup of $G$, and $a \in G$. Then
$$S = \{ n \in \mathbb{Z} : a^n \in H \}$$
is an ideal of $\mathbb{Z}$.*

Let $x, y \in S$, then $a^{x + y} = a^x a^y \in H$ since $H$ is a group. Also $a^x \in H \implies a^{-x} \in H$.

Finally for any $z \in \mathbb{Z}, a^{xz} = \underbrace{(a^x)(a^x)\cdots(a^x)}_{z \text{ times}} \in H$.

So $S = \{ n \in \mathbb{Z}: a^n \in H \}$ is an ideal of $\mathbb{Z}$.

## Q8

*Prove if $\gcd(a, b) = d$, then $\langle a \rangle + \langle b \rangle = \langle d \rangle$.*

Let there be homomorphisms from $\mathbb{Z}$ onto $\langle a \rangle$ and $\langle b \rangle$ defined by
$$\phi(x) = \bar{x}$$
Then $\langle a \rangle \cong \mathbb{Z} / J$ and $\langle b \rangle \cong \mathbb{Z} / K$.

Then $\langle a \rangle + \langle b \rangle = J + K$
$$J + K = \{ x + y : x \in J, y \in K \}$$
All ideals of $\mathbb{Z}$ are principal so there exists a generator $t$ such that $J + K = \langle t \rangle$.

But $t = x + y$ for some $x \in J$ and $y \in K$. And $x = ka$ where $k \in \mathbb{Z}$ and $y = lb$ where $l \in \mathbb{Z}$. Thus $t = ka + lb$.

Since $\gcd(a, b) = d$ and $\langle t \rangle = J + K$ is the set of linear combinations of $a$ and $b$, we know from theorem 3, that $\langle t \rangle$ is an ideal and the $\gcd(a, b)$.

Thus $J + K = \langle d \rangle$ and so
$$\langle a \rangle + \langle b \rangle = \langle d \rangle$$
where $d = \gcd(a, b)$.

# H. The $\gcd$ and the $\lcm$ as Operations on $\mathbb{Z}$

*For any two integers $a$ and $b$, let $a \star b = \gcd(a, b)$ and $a \circ b = \lcm(a, b)$. Prove the following properties of these operations:*

## Q1

*$\star$ and $\circ$ are associative.*

First we prove $(a \star b) \star c = a \star (b \star c)$ or that $\gcd(\gcd(a, b), c) = \gcd(a, \gcd(b, c))$
$$\gcd(a, b) \implies a = a_1 r, b = b_1 r$$
$$\gcd(a, b) = r$$
$$\gcd(\gcd(a, b), c) = \gcd(r, c) \implies r = r_1 u, c = c_1 u$$
$$\gcd(\gcd(a, b), c) = u$$

Now note that $b = b_1 r = b_1 r_1 u$ so
$$\gcd(b, c) = \gcd(b_1 r_1 u, c_1 u) = u$$
and
$$\gcd(a, \gcd(b, c)) = \gcd(a_1 r_1 u, u) = u$$
so
$$(a \star b) \star c = a \star (b \star c)$$

Secondly we prove $(a \circ b) \circ c = a \circ (b \circ c)$ or that $\lcm(\lcm(a, b), c) = \lcm(a, \lcm(b, c))$

Note that $t = \lcm(a, \lcm(b, c))$ then $a \mid t$ and $\lcm(b, c) \mid t$. And $r = \lcm(b, c)$ then $b \mid r$ and $c \mid r$, but also $r \mid t \implies b \mid t$ and $c \mid t$.

Therefore $a \mid t$, $b \mid t$ and $c \mid t$.

Likewise through the same method we can conclude $\lcm(\lcm(a, b), c) \mid \lcm(a, \lcm(b, c))$ and so they are equal.

That is given they are the *least* multiple of $a, b, c$ and so should divide the other value which is also a multiple of $a, b$ and $c$.

From this we conclude they are equal.

We can also use the fact that

\begin{align*}
\lcm(a, \lcm(b, c)) &= \lcm(a, 1^{\max(b_1,c_1)} \cdot 2^{\max(b_2, c_2)} \cdot 3^{\max(b_3, c_3)} \cdot 5^{\max(b_4, c_4)} \cdot 7^{\max(b_5, c_5)} \cdots) \\
&= 1^{\max(a_1, b_1, c_1)} \cdot 2^{\max(a_2, b_2, c_2)} \cdot 3^{\max(a_3, b_3, c_3)} \cdot 5^{\max(a^4, b^4, c^4)} \cdot 7^{\max(a^5, b^5, c^5)} \cdots
\end{align*}

since the $\max$ operation is associative.

## Q2

*There is an identity element for $\circ$, but not for $\star$ (on the set of positive integers).*

Let there be an identity element $e$ for $\star$, then $\gcd(a, e) = a \implies a \mid e$ but also $\gcd(n \cdot a, e) = n \cdot a \implies n \cdot a \mid e$. So every number divides $e$, and it contains every prime number an infinite number of times as its factor.

Thus there is no identity for $a \star b = \gcd(a, b)$.

For the $\lcm$ note that
$$a \circ b = \lcm(a, b) = ab / \gcd(a, b)$$
For the identity operation
$$ae / \gcd(a, e) = \lcm(a, e) = a$$
$$ae = a \gcd(a, e)$$
$$e = \gcd(a, e)$$
So $e$ divides all natural numbers
$$e = 1$$

## Q3

*Which integers have inverses with respect to $\circ$?*

Only $1$ has an inverse because
$$\lcm(a, b) = 1$$
$$\gcd(a, b) = ab / \lcm(a, b) = ab$$
that is
\begin{align*}
a &= a_1 (ab) \\
&= a_1 ((a_1 ab) b) \\
&= a_1 a_1 \cdots b \cdot b
\end{align*}

$$\implies a, b = 1$$

## Q4

*Prove: $a \star (b \circ c) = (a \star b) \circ (a \star c)$.*

\begin{align*}
a \star (b \circ c) &= \gcd(a, \lcm(b, c)) \\
(a \star b) \circ (a \star c) &= \lcm(\gcd(a, b), \gcd(a, c))
\end{align*}

Let $a = a_1fg$, $b = b_1 fx$, and $c = c_1 gx$.

\begin{align*}
\gcd(a, bc/\gcd(b, c)) &= \gcd(a, bc / x) \\
&= gcd(a_1fg, b_1fxc_1gx/x) \\
&= fg
\end{align*}

\begin{align*}
\lcm(\gcd(a, b), \gcd(a, c)) &= \gcd(a, b) \cdot \gcd(a, c) / \gcd(\gcd(a, b), \gcd(a, c)) \\
&= fg / \gcd(f, g) = fg
\end{align*}

