---
title: Abstract Algebra by Pinter, Chapter 23, question B3
author: Amir Taaki
header-includes: |
    - \usepackage{mathrsfs}
    - \usepackage{mathtools}
    - \usepackage{extpfeil}
    - \DeclareMathOperator\ker{ker}
    - \DeclareMathOperator\ord{ord}
    - \DeclareMathOperator\gcd{gcd}
    - \DeclareMathOperator\lcm{lcm}
    - \DeclareMathOperator\mod{mod}
    - \DeclareMathOperator\char{char}
abstract: Chapter 23 on Number Theory
---

# Proof

## Initial Question

*We are given $k$ congruences
$$x \equiv c_1 (\mod m_1) \qquad x \equiv c_2 (\mod m_2) \qquad \cdots \qquad x \equiv (\mod m_k)$$
for all $i, j \in \{1, \dots, k\}$
$$c_i \equiv c_j (\mod d_{ij})$$
where $d_{ij} = \gcd(m_i, m_j)$.*

*Prove there is an $x$ satisfying all $k$ congruences simultaneously, and the solution is of the form
$$x \equiv c (\mod t)$$
where $t = \lcm(m_1, m_2, \dots, m_k)$.*

## Simultaneous Solution for Three Elements

We will proceed to prove these statements through induction, first starting with the case of proving there is a simultaneous solution for $c_1, c_2$ and $c_3$.

It has been shown earlier in theorem 3 that there is a solution for two equations $x \equiv a (\mod n)$ and $x \equiv b (\mod m)$, only exists if
$$a \equiv b (\mod d)$$
$$d = \gcd(m, n)$$

For the first two equations, there is therefore a simultaneous solution because
$$c_1 \equiv c_2 (\mod d_{12})$$

Earlier in theorem 4, it was shown that if $x \equiv a (\mod n)$ and $x \equiv b (\mod m)$ have a simultaneous solution, it is of the form
$$x \equiv c (\mod t)$$
$$t = \lcm(m, n)$$

So therefore the solution of $x \equiv c_1 (\mod m_1)$ and $x \equiv c_2 (\mod m_2)$ is
$$ x \equiv c (\mod t)$$
$$t = \lcm(m_1, m_2)$$

We want to know if there is a solution $x$ for $x = c (\mod t)$ and $x = c_3 (\mod m_3)$. That is whether the statement
$$c_3 \equiv c [\mod \gcd(t, m_3)]$$
is true.

But we know that $\gcd(a, \lcm(b, c)) = \lcm(\gcd(a, b), \gcd(a, c))$ so
\begin{align*}
\gcd(t = \lcm(m_1, m_2), m_3) &= \lcm(\gcd(m_1, m_3), \gcd(m_2, m_3)) \\
&= \lcm(d_{13}, d_{23})
\end{align*}

So we want to know whether this statement is true
\begin{align*}
c_3 &\equiv c [\mod \gcd(t, m_3)] \\
&\equiv c [\lcm(d_{13}, d_{23})]
\end{align*}

At the start it was stated that $c_3 \equiv c_1 (\mod d_{13})$, and we also we know that
$$c \equiv c_1 (\mod m_1) \implies c \equiv c_1 (\mod d_{13})$$
$$\therefore c \equiv c_3 (\mod d_{13})$$
Likewise $c_3 \equiv c_2 (\mod d_{23}) \implies c \equiv c_3 (\mod d_{23})$

Now from the last part of theorem 4, we note that
$$m \mid (x - c) \text{ and } n \mid (x - c) \iff t \mid (x - c)$$
or
$$x \equiv c (\mod m) \text { and } x \equiv c (\mod n) \iff x \equiv c (\mod t)$$

Note that
$$d_{13} \mid (c - c_3) \text { and } d_{23} \mid (c - c_3) \iff lcm(d_{13}, d_{23}) \mid (c - c_3)$$
or
$$c \equiv c_3 (\mod d_{13}) \text{ and } c \equiv c_3 (\mod d_{23}) \iff c \equiv c_3 [\mod \lcm(d_{13}, d_{23})]$$

That is we can state that
$$c_3 \equiv c [\mod \lcm(d_{13}, d_{23})]$$
But $\lcm(d_{13}, d_{23}) = \gcd(t, m_3)$. So by theorem 3 because
$$c_3 \equiv c [\mod \gcd(t, m_3)]$$
there is a simultaneous solution of
\begin{align*}
x &\equiv c (\mod t) \\
x &\equiv c_3 (\mod m_3)
\end{align*}
And this is also the solution for
\begin{align*}
x &\equiv c_1 (\mod m_1) \\
x &\equiv c_2 (\mod m_2)
\end{align*}

## Generalizing to $k + 1$ through induction

Now we will generalize this using induction on $k + 1 \in \mathbb{Z}$ terms where we assume $S_k$ is true, proving the statement $S_{k + 1}$ is true, and therefore it is true for all integers.

Assume there is a solution of $k$ congruences
$$x \equiv c_1 (\mod m_1) \qquad \cdots \qquad x \equiv c_k (\mod m_k)$$
of the form
$$x \equiv c (\mod t)$$
$$t = \lcm(m_1, \dots, m_k)$$

Note that $\forall i, j \in \{1, \dots, k\}$
$$c_i \equiv c_j (\mod d_{ij})$$
$$d_{ij} = \gcd(m_i, m_j)$$
that is
$$c_{k + 1} = c_i (\mod d_{k + 1, i})$$

We want to know if there an $x (\mod t')$ which is the solution for $x \equiv c (\mod t)$ and $x \equiv c_{k + 1} (mod m_{k + 1})$. That is whether the statement
$$c_{k + 1} \equiv c [\mod \gcd(t, m_{k + 1})]$$
is true or not.

## Relation between gcd and lcm operators

From chapter 22, exercise H4, let $a \star b = \gcd(a, b)$ and $a \circ b = \lcm(a, b)$ then it is trivial to show that
$$a \star (b \circ c) = (a \star b) \circ (a \star c)$$
and we know that the $\lcm$ operation is associative.
$$m_1 \circ m_2 \circ \cdots \circ m_k = m_1 \circ (m_2 \circ (\cdots \circ m_k))$$
so
\begin{align*}
m_{k + 1} \star (m_1 \circ m_2 \circ \cdots \circ m_k) &= (m_{k + 1} \star m_1) \circ (m_{k + 1} \star (m_2 \circ \cdots \circ m_k)) \\
&= (m_{k + 1} \star m_1) \circ (m_{k + 1} \star m_2) \circ (m_{k + 1} \star (m_3 \circ \cdots \circ m_k)) \\
&= (m_{k + 1} \star m_1) \circ \cdots \circ (m_{k + 1} \star m_k)
\end{align*}
That is
$$\gcd(\lcm(m_1, \dots, m_k), m_{k + 1}) = \lcm(\gcd(m_1, m_{k + 1}), \dots, \gcd(m_k, m_{k + 1}))$$

## Proving equivalency holds under gcd for $k + 1$

At the beginning it was stated that $\forall i \in \{1, \dots, k\}$
$$c_{k + 1} \equiv c_i (\mod d_{k + 1, i})$$
and we also know that
$$c \equiv c_i (\mod m_i)$$
$$c - c_i = q m_i = q(sd_{k + 1, i})$$
$$\implies c \equiv c_i (\mod d_{k + 1, i})$$

## Generalizing lcm to Multiple Arguments

The $\lcm$ is defined as if $c = \lcm(a, b)$ then

1. $a \mid c$ and $b \mid c$
2. For any $x$ if $a \mid x$ and $b \mid x \implies c \mid x$

This can be generalized for any number of arguments in the $\lcm$ by noting that since $c = \lcm(x_1, x_2, \dots, x_n)$ then $\forall i \in \{1, \dots, n\}$ then 1. $x_i \mid c$ for 2., note that the common multiples of $\{ x_1, \dots, x_n\}$ form an ideal of $\mathbb{Z}$ by $\langle c \rangle = \langle x \rangle \cap \cdots \cap \langle x_n \rangle$, and so every common multiple is a multiple of $c$.

$\therefore$ any $v$ such that $\forall x_i \in X: x_i \mid v \implies c \mid v$.

## Solution $c \equiv c_i$ is also a Solution in the lcm of the gcds

From theorem 4, we generalize that
$$m_1 \mid x, \cdots, m_n \mid x \implies t \mid x$$
$$m_1 \mid (x - c), \cdots, m_n \mid (x - c) \implies t \mid (x - c)$$
$$x \equiv c (\mod m_1) \qquad \cdots \qquad x \equiv c (\mod m_n) \implies x \equiv c (\mod t)$$
where $t = \lcm(m_1, \dots, m_n)$

Now note that
$$d_{k + 1, 1} \mid (c - c_i) \qquad \cdots \qquad d_{k + 1, k} \mid (c - c_i) \implies \lcm(d_{k + 1, 1}, \dots, d_{k + 1, k}) \mid (c - c_i)$$
or
$$c \equiv c_i (\mod d_{k + 1, 1}) \qquad \cdots \qquad c \equiv c_i (\mod d_{k + 1, k}) \implies c \equiv c_i [\mod \lcm(d_{k + 1, 1}, \dots, d_{k + 1, k})]$$

## There is a Common Solution for $c$ and $c_{k + 1}$

So,
$$c \equiv c_i [\mod \lcm(\gcd(m_{k + 1}, m_1), \dots, \gcd(m_{k + 1}, m_k))]$$

But we know that
$$\lcm(\gcd(m_{k + 1}, m_1), \dots, \gcd(m_{k + 1}, m_k)) = \gcd(\lcm(m_1, \dots, m_k), m_{k + 1})$$
$$\implies c \equiv c_i [\mod \gcd(t, m_{k + 1})]$$
where $t = \lcm(m_1, \dots, m_k)$

And because of this, by theorem 3, because $\forall i \in \{1, \dots, k\}, c \equiv c_i [\mod \gcd(t, m_{k + 1})]$, there is an $x$ such that
$$x \equiv c (\mod t)$$
$$x \equiv c_{k + 1} (\mod m_{k + 1})$$
which because $x \equiv c (\mod t)$, this is also the solution for
$$x \equiv c_1 (\mod m_1)$$
$$\cdots$$
$$x \equiv c_k (\mod m_k)$$

Furthermore this solution takes the form
\begin{align*}
x &\equiv c' [\mod \lcm(t, m_{k + 1})] \\
&\equiv c' (\mod t')
\end{align*}
where $t' = \lcm(m_1, m_2, \dots, m_k)$

