---
title: Abstract Algebra by Pinter, Chapter 23
author: Amir Taaki
header-includes: |
    - \usepackage{mathrsfs}
    - \usepackage{mathtools}
    - \usepackage{extpfeil}
    - \DeclareMathOperator\ker{ker}
    - \DeclareMathOperator\ord{ord}
    - \DeclareMathOperator\gcd{gcd}
    - \DeclareMathOperator\lcm{lcm}
    - \DeclareMathOperator\char{char}
    - \DeclareMathOperator\max{max}
    - \newcommand{\mod}[1]{\ (\mathrm{mod}\ #1)}
abstract: Chapter 23 on Elements of Number Theory
---

# A. Solving Single Congruences

## Q1

### a

$$ 60x \equiv 12 \mod{24} $$
$$ \gcd(60, 24) = 12/12 $$
$$ \implies 5x \equiv 1 \mod 2 $$
$$ x \equiv 3 \mod 2 $$

### b

$$ \gcd(42, 30) = 6 $$
$$ 7x \equiv 4 \mod 5 $$
$$ x \equiv 2 \mod 5 $$

### c

No solution because $\gcd(49, 25) = 1$ so equation cannot be reduced.

### d

$$ 39 = 13 \times 3 $$
$$ 52 = 13 \times 2^2 $$
$$ \gcd(39, 52) = 13 \nmid 14 $$

### e

$$ \gcd(147, 98) = 49 \nmid 47 $$

### f

$$ \gcd(39, 52) = 13 $$
$$ 3x \equiv 2 \mod 4 $$
$$ x \equiv 3 $$

## Q2

### a

$$ 12x \equiv 7 \mod{25} $$
Note that $12 \perp 25$
$$ 12k + 25l = 1 $$
$$ \implies k = -2, l = 1 $$
$$ \implies 12 \cdot (-2) \equiv 1 \mod{25} $$
$$ \implies 12 \cdot 23 \equiv 1 \mod{25} $$
$$ \implies 12 \cdot 23 \cdot 7 \equiv 7 \mod{25} $$
$$ \implies 12 \cdot 11 \equiv 7 \mod{25} $$

### b

$$ 35x \equiv 8 \mod{12} $$
$$ 35 \perp 12 $$
$$ \implies 35 \cdot (-1) + 12 \cdot 3 = 1 $$
$$ \implies 35 \cdot (-1) \equiv 1 \mod{12} $$
$$ \implies 35 \cdot 11 \equiv 1 \mod{12} $$
$$ \implies 35 \cdot 88 \equiv 8 \mod{12} $$
$$ \implies 35 \cdot 4 \equiv 8 \mod{12} $$

### c

$$ 15x \equiv 9 \mod 6 $$
$$ 15k + 6l = 1 $$
$$ 15 = 6(2) + 3 $$
$$ 6 = 3(2) + 0 $$
$$ \gcd(15, 6) = 3 $$
$$ 5x \equiv 3 \mod 2 $$
$$ x \equiv 1 \mod 2 $$
$$ 15(1) \equiv 9 \mod 6 $$

### d

$$ 42x \equiv 12 \mod{30} $$
$$ 42k + 30l = \gcd(42, 30) $$
$$ 42 = 30(1) + 12 $$
$$ 30 = 12(2) + 6 $$
$$ 12 = 6(2) + 0 $$
$$ 7x \equiv 2 \mod 5 $$
$$ 2x \equiv 2 \mod 5 $$
$$ x \equiv 1 \mod 5 $$
$$ x \equiv 1 \mod{30} $$

### e

$$ 147x \equiv 49 \mod{98} $$
$$ \bar{147} = \bar{49} $$
$$ \implies 49x \equiv 49 \mod{98} $$
$$ \implies x \equiv 1 \mod{98} $$

### f

$$ 39x \equiv 26 \mod{52} $$
$$ 52 = 39(1) + 13 $$
$$ 39 = 13(3) + 0 $$
$$ \implies \gcd(52, 39) = 13 $$
$$ \implies 3x \equiv 2 \mod 4 $$
$$ \implies x \equiv 2 \mod 4 $$
$$ \implies x \equiv 2 \mod{52} $$

## Q3

### a

$$ 2x^2 \equiv 8 \mod{10} $$
$$ \implies 2x^2 - 8 = 10y $$
but $\gcd(2, 10) = 2$
$$ \implies x^2 - 4 = 5y \in \langle 5 \rangle $$
$$ \implies x^2 - 4 \equiv 0 \mod 5 $$
$$ \implies x^2 \equiv 4 \mod{10} $$

### b

$$ 1^2 \equiv 1 \mod 5 $$
$$ 2^2 \equiv 4 \mod 5 $$
$$ 3^2 \equiv 4 \mod 5 $$
$$ 4^2 \equiv 1 \mod 5 $$

## Q4

### a

$$ 6x^2 \equiv 9 \mod{15} \implies 2x^2 \equiv 3 \mod 5 $$
$$ \implies x = 2 \mod 5 $$

### b

$$ 60x^2 \equiv 18 \mod{24} \implies 10x^2 \equiv 3 \mod 4 $$
$$ \implies 2x^2 \equiv 3 \mod 4 $$

$x \neq 2$ because $2 \times 2 \mid 4 \implies x^2 \equiv 0 \mod 4$.

Likewise coefficient is 2 so for any $n$, $2n$ is either 2 or 0. No solution.

### c

$$ 30x^2 \equiv 18 \mod{24} $$
$$ \implies 5x^2 \equiv 3 \mod 4 $$
$$ \implies x^2 \equiv 3 \mod 4 $$
No solution.

### d

$$ 4(x + 1)^2 \equiv 14 \mod {10} $$
$$ \implies 4(x + 1)^2 \equiv 4 \mod {10} $$
$$ x \equiv 0 \mod {10} $$

### e

$$ 4x^2 - 2x + 2 \equiv 0 \mod 6 $$
$$ \implies 2x^2 - x + 1 \equiv 0 \mod 3 $$
$$ \implies x = 2 $$

### f

$$ 3x^2 - 6x + 6 \equiv 0 \mod {15} $$
$$ \implies x^2 - 2x + 2 \equiv 0 \mod 5 $$
$$ x = 3, 4 \mod 5 $$

## Q5

### a

$$ x^4 \equiv 4 \mod 6 $$
$$ x^4 \equiv (x^2)^2 \mod 6 $$
Let $y = x^2$
$$y^2 \equiv 4 \mod 6 $$
$$y \equiv 2 \mod 6 \text{ or } 4 \mod 6 $$
$$x^2 = 2 \mod 6 \text { or } 4 \mod 6 $$
$$\implies x \equiv 2 \mod 6 $$

### b

$$2(x - 1)^4 \equiv 0 \mod 8 $$
$$\implies (x - 1)^4 \equiv 0 \mod 4 $$
$$\implies (x - 1)^2 \equiv 0, 2 \mod 4 $$
Let $y = x - 1$
$$\implies y^2 \equiv 0 \mod 4 $$
$$ \implies y \equiv 0, 2 \mod 4 $$
$$ \implies x \equiv 1, 3 \mod 4 $$

### c

$$ x^3 + 3x^2 + 3x + 1 \equiv 0 \mod 8 $$
$$ (x + 1)^3 \equiv 0 \mod 8 $$
$$ \implies x + 1 \equiv 0, 2, 4, 6 $$
(any factor of 2 since $2^3 \equiv 8 \equiv 0$)
$$ \implies x \equiv 7, 1, 3, 5 $$

### d

$$ x^4 + 2x^2 + 1 \equiv 4 \mod 5 $$
$$ \implies (x^2 + 1) \equiv 4 \mod 5 $$
$$ \implies x^2 + 1 \equiv 2, 3 \mod 5 $$
$$ \implies x^2 \equiv 1, 2 \mod 5 $$
$$ \implies x \equiv 1, 4 \mod 5 $$

## Q6

### a

$$ 14x + 15y = 11 $$
Note that $14(-1) + 15(1) = 1$, thus
$$14(-1 \cdot 11) + 15(1 \cdot 11) = 11$$
$$x = -11, y = 11$$

### b

$$4(-1) + 5(1) = 1$$

### c

$21x + 10y$ is an ideal in $\mathbb{Z}$, with a least value $t$, such that $J = \langle t \rangle$ and therefore if $q \in J$ then $t \mid q$.

But the least value $t = 11$ and $11 \nmid 9$. So there is no solution.

### d

$$30x^2 + 24y = 18$$
$$30x^2 \equiv 18 \mod{24} $$
$$ 5x^2 \equiv 3 \mod 4 $$
$$ x^2 \equiv 3 \mod 4 $$

# B. Solving Sets of Congruences

## Q1

### a

$$x \equiv 7 \mod 8 \qquad x \equiv 11 \mod {12} $$
$$\gcd(8, 12) = 4$$
$$7 \mod 4 \equiv 3 \equiv 11 \mod 4 $$
Solution exists.
$$ \lcm(8, 12) = 8 \times 12 / 4 = 24 $$

$$x = 8q + 7 $$
$$ \implies 8q + 7 \equiv 11 \mod{12} $$
$$ 8q \equiv 4 \mod{12}$$
\begin{align*}
q &\equiv 5 \mod {12} \\[8pt]
x &= 8q + 7 \\
&= 8(12r + 5) + 7 \\
&= 96r + 47 \\[8pt]
x &\equiv 47 \mod{24} \\
&\equiv 23 \mod{24}
\end{align*}

### b

$$ x \equiv 12 \mod{18} \qquad x \equiv 30 \mod{45} $$
$$ \gcd(18, 45) = 9 $$
$$ \lcm(18, 45) = 18 \times 45 / 9 = 90 $$

$$ x = 18q + 12 $$

\begin{align*}
18q + 12 &\equiv 30 \mod{45} \\
18q &\equiv 18 \mod{45} \\
q &\equiv 1 \mod{45} \\[8pt]
x &= 18(45r + 1) + 12 \\
&= 18 \times 45 r + 30 \\
x &\equiv 30 \mod{90}
\end{align*}

### c

\begin{align*}
\gcd(15, 14) &= 1 \\
\lcm(15, 14) &= 210
\end{align*}

\begin{align*}
15q + 8 &\equiv 11 \mod{14} \\
15q &\equiv 3 \mod{14} \\
q &\equiv 3 \mod{14} \\[8pt]
x &\equiv 53 \mod{210}
\end{align*}

## Q2

### a

$$ 10x \equiv 2 \mod{12} \qquad 6x \equiv 14 \mod{20} $$
$$ \gcd(10, 12) = 2 $$
\begin{align*}
5x &\equiv 1 \mod 6 \\
x &\equiv 5 \mod 6 \\[8pt]
6x &\equiv 14 \mod{20} \\
3x &\equiv 7 \mod{10} && \gcd(6, 20) = 2 \\
x &\equiv 9 \mod{10}
\end{align*}
\begin{align*}
\gcd(6, 10) &= 2 \\
5 \mod 2 &= 1 = 9 \mod 2
\end{align*}
has a solution.
$$ \lcm(6, 10) = 30 $$
solution is modulo 30.

$$ x = 6q + 5 $$
\begin{align*}
6q + 5 &\equiv 9 \mod{10} \\
6q &\equiv 4 \mod{10} \\
3q &\equiv 2 \mod 5 && [\text{from } \frac{a}{d} x \equiv \frac{b}{d} \mod{\frac{c}{d}}] \\
q &\equiv 4 \mod 5 \\[8pt]
q &= 5r + 4
\end{align*}
$$ x = 6(5r + 4) + 5 = 30r + 29 $$
$$ x \equiv 29 \mod{30} $$

### b

\begin{align*}
4x &\equiv 2 \mod 6 \\
9x &\equiv 3 \mod{12}
\end{align*}
$$ \gcd(4, 6) = 2 $$
$$ \therefore 4x \equiv 2 \mod 6 \implies 2x \equiv 1 \mod 3 $$
$$ x \equiv 2 \mod 3 $$

$$ \gcd(9, 12) = 3 $$
$$ \therefore 9x \equiv 3 \mod{12} \implies 3x \equiv 1 \mod 4 $$
$$x \equiv 3 \mod 4 $$
$$ \gcd(3, 4) = 1 $$
$$ 2 \mod 1 = 0 \neq 3 \mod 1 $$
has no solution.

### c

\begin{align*}
6x &\equiv 2 \mod 8 \\ 
10x &\equiv 2 \mod{12}
\end{align*}
\begin{align*}
\gcd(6, 8) &= 2 \implies 3x \equiv 1 \mod 4 \\
\gcd(10, 12) &= 2 \implies 5x \equiv 1 \mod 6
\end{align*}
$$ \implies x \equiv 3 \mod 4 $$
$$ \implies x \equiv 5 \mod 6 $$
$$ \gcd(4, 6) = 2 $$
$$ 3 \mod 2 = 1 = 5 \mod 2 $$
has a solution.
$$ \lcm(4, 6) = 12 $$
$$ x = 4q + 3 $$
\begin{align*}
4q + 3 &\equiv 5 \mod 6 \\
4q &\equiv 2 \mod 6
\end{align*}
$$ \gcd(4, 6) = 2 $$
$$ \implies 2q \equiv 1 \mod 3 $$
$$ q \equiv 2 \mod 3 $$
$$q = 3r + 2 $$
\begin{align*}
x &= 4(3r + 2) + 3 \\
&= 12r + 11 \\
x &\equiv 11 \mod{12}
\end{align*}

## Q3

See attached file `ch23b3.pdf`.

## Q4

### a

$$x \equiv 2 \mod 3 \qquad x \equiv 3 \mod 4 \qquad x \equiv 1 \mod 5 \qquad x \equiv 4 \mod 7$$
All modulo are coprime so there is a solution.
$$\lcm(3, 4, 5, 7) = 3 \times 4 \times 5 \times 7 = 420 $$
recursively find a solution for each equation.
$$x = 3q + 2 $$
\begin{align*}
3q + 2 &\equiv 2 \mod 4 \\
3q &\equiv 1 \mod 4 \\
q &\equiv 3 \mod 4
\end{align*}
$$ q = 4r + 3 $$
\begin{align*}
x &= 3(4r + 3) + 2 \\
&= 12r + 11 \\
x &\equiv 11 \mod{12}
\end{align*}
but also $x \equiv 1 \mod 5$
$$x = 12q' + 11$$
\begin{align*}
12q' + 11 &\equiv 1 \mod 5 \\
12q' &\equiv 0 \mod 5 \\
q' &\equiv 0 \mod 5 \\
q' &= 5r' \\
\implies x &= 11
\end{align*}
this also fits the equation $x \equiv 4 \mod 7$.

### b

$$ 6x \equiv 4 \mod 8 \qquad 10x \equiv 4 \mod{12} \qquad 3x \equiv 8 \mod{10} $$

$$6x \equiv 4 \mod 8 \implies 3x \equiv 2 \mod 4 \implies x \equiv 2 \mod 4 $$
$$10x \equiv 4 \mod{12} \implies 5x \equiv 2 \mod 6 \implies x \equiv 4 \mod 6 $$
$$ 3x \equiv 8 \mod{10} \implies x \equiv 6 \mod{10} $$

$$ \gcd(4, 6) = 2 \qquad 2 \mod 2 = 0 = 4 \mod 2 $$
$$ \gcd(4, 10) = 2 \qquad 2 \mod 2 = 0 = 6 \mod 2 $$
$$ \gcd(6, 10) = 2 \qquad 2 \mod 2 = 0 = 6 \mod 2 $$
thus there is a solution $x$.
$$t = \lcm(4, 6, 10) = \lcm(\lcm(4, 6), 10) = \lcm(12, 10) = 60 $$
Solution is modulo $t = 60$.

\begin{align*}
x &\equiv 2 \mod 4 \\
x &\equiv 4 \mod 6 \\
x &\equiv 6 \mod{10} \\[8pt]
x &= 4q + 2 \\[8pt]
4q + 2 &\equiv 4 \mod 6 \\
4q &\equiv 2 \mod 6 \\
q &\equiv 2 \mod 6 \\
q &= 6r + 2 \\[8pt]
x &= 4(6r + 2) + 2 \\
&= 24r + 10
\end{align*}
\begin{align*}
24r + 10 &\equiv 6 \mod{10} \\
24r &\equiv -4 \mod{10} \\
&\equiv 6 \mod{10} \\
12r &\equiv 3 \mod 5 \\
r \equiv 4 \mod 5 \\
r = 5s + 4
\end{align*}
\begin{align*}
x &= 24(5s + 4) + 10 \\
&= 120s + 106 \\
x &= 106 \mod{60} \\
&= 46 \mod{60}
\end{align*}

## Q5

### a

$$ 4x + 6y = 2 \implies 4x \equiv 2 \mod 6 $$
$$ 9x + 12y = 3 \implies 9x \equiv 3 \mod{12} $$

$$4x \equiv 2 \mod 6 \implies 2x \equiv 1 \mod 3 \implies x \equiv 2 \mod 3 $$
$$ 9x \equiv 3 \mod{12} \implies 3x \equiv 1 \mod 4 \implies x \equiv 3 \mod 4 $$

$$x = 3q + 2 $$
\begin{align*}
3q + 2 &\equiv 3 \mod 4 \\
3q &\equiv 1 \mod 4 \\
q &\equiv 3 \mod 4
\end{align*}
$$ q = 4r + 3 $$
\begin{align*}
x &= 3(4r + 3) + 2 \\
&= 12r + 11
\end{align*}
$$t = \lcm(6, 12) = 12$$
$$x \equiv 11 \mod{12}$$
\begin{align*}
x &= 12s + 11 \\
&= -1 \\
y &= 1
\end{align*}

### b

\begin{align*}
3x + 4y &= 2 \\
5x + 6y &= 2 \\
3x + 10y &= 8
\end{align*}

\begin{align*}
3x &\equiv 2 \mod 4 \\
5x &\equiv 2 \mod 6 \\
3x &\equiv 8 \mod 10
\end{align*}

From 23B4b, $x \equiv 46 \mod{60}$

\begin{align*}
6y &\equiv 2 \mod 5 \\
y &\equiv 2 \mod 5 \\[8pt]
10y &\equiv 8 \mod 3 \\
y &\equiv 2 \mod 2 \\[8pt]
4y &\equiv 2 \mod 3 \\
y &\equiv 2 \mod 3
\end{align*}

$$ t = \lcm(3, 5) = 15 $$
$$ y = 5q + 2 $$

\begin{align*}
5q + 2 &\equiv 2 \mod 3 \\
2q &\equiv 0 \mod 3 \\[8pt]
y &= 2
\end{align*}
but $x \equiv 46 \mod{60}$
\begin{align*}
5(46) + 6(2) &\equiv 50 + 12 \equiv 2 \mod {60} \\
3(46) + 10(2) &\equiv 18 + 20 \equiv 38 \not\equiv 8 \mod {60}
\end{align*}
so there's no solution.

# C. Elementary Properties of Congruence

## Q1

*If $a \equiv b \mod n$ and $b \equiv c \mod n$, then $a \equiv c mod n$.*

$$ b - a = nq_1 $$
$$ b = nq_1 + a $$
$$ b - c = nq_2 $$
$$(nq_1 + a) - c = nq_2 $$
\begin{align*}
a - c &= nq_2 - nq_2 \\
&= n(q_2 - q_1)
\end{align*}
$$ \implies a \equiv c \mod n $$

## Q2

*If $a \equiv b \mod n$, then $a + c \equiv b + c \mod n$.*

$$ a - b = nq $$
$$ c - c = 0 $$
$$a - b + (c - c) = nq $$
$$(a + c) - (b + c) = nq $$
$$ \implies a + c \equiv b + c \mod n $$

## Q3

*If $a \equiv b \mod n$, then $ac \equiv bc \mod n$.*

$$a - b = nq $$
$$c(a - b) = cnq $$
$$ac - ab = n(qc) $$
$$ac \equiv bc \mod n $$

## Q4

*$a \equiv b \mod 1$.*

$$a \equiv b \mod n \iff n \mid (a - b) $$
$$1 \mid (a - b) \implies a \equiv b \mod 1 $$

## Q5

*If $ab \equiv 0 \mod p$, where $p$ is a prime, then $a \equiv 0 \mod p$ or $b \equiv 0 \mod p$.*

$$ab \equiv 0 \mod p \implies ab = np $$
$$ \implies p \mid ab $$
but $p$ is prime so either $p \mid a$ or $p \mid b$.

If $p \mid a$ then $a \equiv 0 \mod p$.

If $p \mid b$ then $b \equiv 0 \mod p$.

## Q6

*If $a^2 \equiv b^2 \mod p$, where $p$ is a prime, then $a \equiv \pm b \mod p$.*

$$a^2 \equiv b^2 \mod p$$
$$a^2 - b^2 = np$$
$$(a + b)(a - b) = np$$
Since $p$ is prime then either $p \mid (a + b)$

If $p \mid (a + b)$ then $a \equiv -b \mod p$.

If $p \mid (a - b)$ then $a \equiv b \mod p$.

## Q7

*If $a \equiv b \mod m$, then $a + km \equiv b \mod m$, for any integer $k$. In particular, $a + km \equiv a \mod m$.*

$$a \equiv b \mod m \implies a - b = mq_1$$
\begin{align*}
\implies (a + km) - b &= mq_1 + km \\
&= m(q_1 + k)
\end{align*}
$$ \implies a + km \equiv b \mod m $$
$$ a - a = 0 = 0m \implies a \equiv a \mod m $$
$$ \implies a + km \equiv a \mod m $$

## Q8

*If $ac \equiv bc \mod n$ and $\gcd(c, n) \equiv 1$, then $a \equiv b \mod n$.*

$$ac \equiv bc \mod n \implies ac - bc = c(a - b) = nq$

So $n \mid c(a - b)$ but $\gcd(c, n) = 1 \implies n \mid (a - b) \implies a \equiv b \mod n$.

## Q9

*If $a \equiv b \mod n$, then $a \equiv b \mod m$ for any $m$ which is a factor of $n$.*

$$n = rm$$
\begin{align*}
a - b &= nq = (rm) q \\
&= m(rq)
\end{align*}
$$ \implies a \equiv b \mod m $$

# D. Further Properties of Congruence

## Q1

*If $ac \equiv bc \mod n$, and $\gcd(c, n) \equiv d$, then $a \equiv b \mod n/d$.*

$$ ac - bc = nq $$
$$ \gcd(c, n) = d \implies c = c_1 d, n = n_1 d $$
$$ c_1 d (a - b) = n_1 d q $$
$$ c_1 (a - b) = n_1 q $$
but $\gcd(c_1, n_1) = 1$ so $n_1 \nmid c_1 \implies n_1 \mid (a - b)$.

$$ \implies a - b = n_1 k $$
$$ n = n_1 d \implies n_1 = \frac{n}{d} $$
$$ a - b = (\frac{n}{d})k $$
$$ \implies a \equiv b \mod{\frac{n}{d}}$$

## Q2

*If $a \equiv b \mod n$, then $\gcd(a, n) = \gcd(b, n)$.*

$$a_1 d \equiv b \mod {n_1 d}$$
$$a_1 d - b = n_1 dy $$
\begin{align*}
b &= a_1 d - n_1 dy \\
&= d(a_1 - n_1 y)
\end{align*}
$$\implies d \mid b $$
$$ \gcd(a_1, n_1) = 1 \implies \gcd(b, n_1) = 1 $$
$$ \implies \gcd(b, n) = d $$

## Q3

*If $a \equiv b \mod p$ for every prime $p$, then $a \equiv b$.*

Assume $a \neq b$ and
\begin{align*}
a &= p_1 \cdots p_i p_{i + 1} \cdots p_n \\
b &= p_1 \cdots p_i q_i \cdots q_m
\end{align*}
where $\gcd(a, b) = p_1 \cdots p_i$.

If $p \in \{ p_1, \dots, p_i \}$ then $p \mid a$ and $p \mid b$ and $a \mod p \equiv 0 \equiv b \mod p$.

If $p \in \{ q_1, \dots, q_m \}$ where $p \neq p_j$ such that $1 \leq j \leq n$ then $p \nmid a$ and $p \nmid b$ so $a \not\equiv b \mod p$.

Likewise for $p = p_j : i \leq j \leq n$.

Therefore $a \equiv b \mod p$ for all prime $p$ implies they both share the exact same prime factors, and $a = b$.

## Q4

*If $a \equiv b \mod n$, then $a^m \equiv b m \mod n$ for every positive integer $m$.*

$$(a - b) = nq$$
\begin{align*}
a &= b + nq \\
a^m &= (b + nq)^m \\
&= b^m + \binom{1}{m} b^{m - 1} (nq)^1 + \cdots + \binom{m - 1}{m}b(nq)^{m - 1} + (nq)^m
\end{align*}
$$ \implies a^m \equiv b^m \mod n$$

## Q5

*If $a \equiv b \mod m$ and $a \equiv b \mod n$ where $\gcd(m, n) = 1$, then $a \equiv b \mod mn$.*

$$a - b = mx = ny$$
$$ \implies n \mid (a - b) \text{ and } m \mid (a - b)$$

but $\gcd(m, n) = 1 \implies mn \mid (a - b)$
$$a \equiv b \mid {mn}$$

## Q6

*If $ab \equiv 1 \mod c$, $ac \equiv 1 \mod b$ and $bc \equiv 1 \mod a$, then $ab + bc + ac \equiv 1 \mod abc$. (Assume $a, c > 0$.)*

\begin{align*}
ab - 1 &= cq_1 \\
ac - 1 &= bq_2 \\
bc - 1 &= aq_3
\end{align*}

$$(ab - 1)(ac - 1)(bc - 1) = (abc)(q_1 q_2 q_3)$$

$$(a^2bc - ab - ac + 1)(bc - 1) = a^2b^2c^2 - ab^2c - abc^2 + bc - a^2bc + ab + ac - 1$$
$$(a^2b^2c^2 - ab^2c - abc^2 - a^2bc) + bc + ab + ac \equiv 1 \mod {abc} $$
$$\implies ab + bc + ac \equiv 1 \mod {abc} $$

## Q7

*If $a^2 \equiv 1 \mod 2$, then $a^2 \equiv 1 \mod 4$.*

$$a^2 - 1 \mid 2 \implies a^2 - 1 \mid 4$$

## Q8

*If $a \equiv b \mod n$, then $a^2 + b^2 \equiv 2ab \mod {n^2}$, and conversely.*

$$a - b = nq$$
$$(a - b)^2 = a^2 - 2ab + b^2 = n^2 q^2$$
$$ \implies a^2 + b^2 = 2ab \mod{n^2} $$

## Q9

*If $a \equiv 1 \mod m$, then $a$ and $m$ are relatively prime.*

$$a - 1 = mq$$
$$a - mq = 1$$

From 22c1 this implies $\gcd(a, b) = 1$.

# E. Consequences of Fermat's Theorem

## Q1

*If $p$ is a prime, find $\phi(p)$. Use this to deduce Fermat's theorem from Euler's theorem.*

$V_p$ is the set of all invertible elements in $\mathbb{Z}_p$.

$V_p$ is thus a group with respect to multiplication.

Let $\bar{a} \in V_p$

$$\bar{sa} = 1$$
$$ \implies sa - 1 \in \langle n \rangle $$
$$ \implies sa - 1 = tn $$
$$sa - tn = 1$$

So invertible elements $a$ in $\mathbb{Z}_n \implies a$ and $n$ are relatively prime, and vice versa.

All cosets of $\langle n \rangle$ (except $\langle n \rangle$ itself) have a $\gcd$ of 1.
$$\mathbb{Z}_p^* = \{ \bar{1}, \bar{2}, \dots, \bar{p - 1} \}$$
So it follows that
$$\phi(p) = p - 1$$

## Q2

*If $p > 2$ is a prime and $a \neq 0 \mod p$, then*
$$a (p - 1)/2 \equiv \pm 1 \mod p$$

$$a^{p - 1} = 1 \mod p$$
$$\implies a^{\frac{p - 1}{2} \cdot 2} \equiv x^2 \equiv 1 \mod p $$
$$x^2 \equiv 1 \mod p \implies x \in \{ -1, 1 \}$$

$$a^{(p - 1)/2} \equiv \pm 1 \mod p$$

## Q3

## a

*Let $p$ be a prime $> 2$. If $p \equiv 3 \mod 4$, then $(p - 1)/2$ is odd.*

$$p \equiv 3 \mod 4$$
$$p - 1 \equiv 2 \mod 4 $$
$$\implies 4 \mid [(p - 1) - 2]$$
$$\implies (p - 1) - 2 = 4q $$
$$\implies \frac{p - 1}{2} - 1 = 2q$$
$$\implies \frac{p - 1}{2} \equiv 1 \mod 2$$
thus $\frac{p - 1}{2}$ is odd.

## b

*Let $p > 2$ be a prime such that $p \equiv 3 \mod 4$. Then there is no solution to the congruence $x^2 + 1 \equiv 0 \mod p$*.

$$x^2 \equiv -1 \mod p$$
$$x^{2 \cdot \frac{p - 1}{2}} \equiv (-1)^{\frac{p - 1}{2}} \mod p$$
By Fermat's theorem
$$ x^{p - 1} \equiv 1 \mod p $$
but since $(p - 1) / 2$ is odd, then $(-1)^{\frac{p - 1}{2}} = -1$ so there is no solution to the congruence $x^2 + 1 \equiv 0 \mod p$.

## Q4

*Let $p$ and $q$ be distinct primes. Then $p^{q - 1} + q^{p - 1} \equiv 1 \mod {pq}$*.

\begin{align*}
p^{q - 1} &\equiv 1 \mod q \\
q^{p - 1} &\equiv 1 \mod p
\end{align*}
\begin{align*}
p^{q - 1} - 1 &= qn \\
q^{p - 1} - 1 &= pm
\end{align*}
\begin{align*}
(p^{q - 1} - 1)(q^{p - 1} - 1) &= p^{q - 1}q^{p - 1} - p^{q - 1} - q^{p - 1} + 1 \\
&= (pq)(mn)
\end{align*}
$$ \implies p^{q - 1} + q^{p - 1} \equiv 1 \mod{pq} $$

## Q5

Let $p$ be a prime.

### a

*If, $(p - 1) \mid m$, then $a^m \equiv 1 \mod p$ provided that $p \nmid a$.*

$$(p - 1) \mid m \implies m = q(p - 1)$$
$$a^m = a^{q(p - 1)} = (a^{p - 1})^q$$

$$a^{p - 1} \equiv 1 \mod p$$
$$(a^{p - 1})^q \equiv 1^q \mod p$$
$$a^m \equiv 1 \mod p$$

### b

*If, $(p - 1) \mid m$, then $a^m + 1 \equiv a \mod {pq}$ for all integers $a$.*

If $p \mid a$ then $a^x \equiv 0 \mod p$ for any $x$ so $a^{m + 1} \equiv 0 \equiv a \mod p$.

Otherwise $p \nmid a$ so $a^m \equiv 1 \mod p \implies a^{m + 1} \equiv a \mod p$

## Q6

*Let $p$ and $q$ be distinct primes.*

### a

*If $(p - 1) \mid m$ and $(q - 1) \mid m$, then $a^m \equiv 1 \mod {pq}$ for any $a$ such that $p \nmid a$ and $q \nmid a$.*

\begin{align*}
a^m &\equiv 1 \mod p \\
a^m &\equiv 1 \mod q
\end{align*}

$$ \gcd(p, q) = 1 \implies p \text{ and } q \text{ share no divisors} $$

but $p \mid (a^m - 1)$ and $q \mid (a^m - 1) \implies pq \mid (a^m - 1)$

\begin{align*}
a^m - 1 &\equiv 0 \mod {pq} \\
a^m &\equiv 1 \mod {pq}
\end{align*}

### b

*If $(p - 1) \mid m$ and $(q - 1) \mid m$, then $a^m + 1 \equiv a \mod {pq}$ for integers $a$*.

Let $p \mid a$ then $a \equiv 0 \mod p$ and $a \equiv 1 \mod q$.

$$\implies a^m (a - 1) = (pq)(mn) $$
$$\implies a^{m + 1} - a = (pq)(mn) $$
$$ \implies a^{m + 1} \equiv a \mod {pq} $$

Likewise if $q \mid a$.

If both $p \mid a$ and $q \mid a$ then $pq \mid a$ and so $a \equiv 0 \mod {pq}$ and $a^{m + 1} \equiv 0 \mod{pq}$.

Otherwise $p \nmid a$ and $q \nmid a$ so
$$a^m \equiv 1 \mod{pq}$$
$$\implies a^{m + 1} \equiv a \mod {pq}$$

## Q7

$$\forall i \in \{ 1, \dots, n \}, (p_i - 1) \mid m$$
$$ \implies a^{m + 1} \equiv a \mod {\prod_{i=1}^n p_i} $$

## Q8

### a

$$p = 7 \qquad q = 19 \qquad m = 18$$
$$(7 - 1) \mid 18 \qquad (19 - 1) \mid 18$$
$$\implies a^{18 + 1} = a \mod {7 \times 19} $$
$$a^19 \equiv a \mod {133}$$

### b

$$a \in \langle 2 \rangle, \langle 3 \rangle, \langle 11 \rangle$$

$$m = 10$$
$$q_1 = 2 \qquad q_2 = 3 \qquad q_3 = 11$$
$$ \implies a^{10} = 1 \mod {66}$$

### c

$$q_1 = 5 \qquad q_2 = 17 \qquad q_3 = 3 $$
$$m = 12$$
$$(5 - 1) \mid 12 \qquad (7 - 1) \mid 12 \qquad (3 - 1) \mid 12$$
$$ \implies a^{13} \equiv a \mod{105}$$

### d

$$q_1 = 7 \qquad q_2 = 13 \qquad q_3 = 17$$
$$m = 48$$
$$(7 - 1) \mid 48 \qquad (13 - 1) \mid 48 \qquad (17 - 1) \mid 48$$
$$\implies a^{49} \equiv a \mod {1457}$$

## Q9

### a

$$ Q = \{ 2, 3, 5, 7 \}$$
$$8^{38} = 8^{2 \times 19} = (8^2)^19 $$
$$\forall q \in Q, (q - 1) \mid (19 - 1)$$
$$ \implies a^{18 + 1} \equiv a \mod{210}$$
where $a = 8^2$
$$\implies x = 8^2$$

### b

$$p = 7 \qquad q = 19$$
$$7^{57} = (7^3)^19$$
$$m = 18$$
$$(7 - 1) \mid m \qquad (19 - 1) \mid m$$
$$a^{m + 1} \equiv a \mod{pq}$$
$$(7^3)^{18 + 1} \equiv 7^3 \mod {7 \times 19}$$
$$ x = 7^3$$

### c

$$Q = \{2, 3, 11 \}$$
$$72 = 2^3 3^2 $$
$73$ is prime so $m \neq 73$ since there is no $(p - 1) \mid m : p \in Q$.

Since $(p - 1) \mid m$ then $m = 72$, if $p = 11$ then $(11 - 1) \nmid 72$ so $m \neq 72$.

Since 5 is a prime, and there are no factorizations of 73, this has no solution.
