---
title: Abstract Algebra by Pinter, Chapter 24
author: Amir Taaki
header-includes: |
    - \usepackage{mathrsfs}
    - \usepackage{mathtools}
    - \usepackage{extpfeil}
    - \DeclareMathOperator\ker{ker}
    - \DeclareMathOperator\ord{ord}
    - \DeclareMathOperator\gcd{gcd}
    - \DeclareMathOperator\lcm{lcm}
    - \DeclareMathOperator\char{char}
    - \DeclareMathOperator\max{max}
    - \DeclareMathOperator\ran{ran}
    - \DeclareMathOperator\deg{deg}
    - \newcommand{\mod}[1]{\ (\mathrm{mod}\ #1)}
    - \newcommand{\repr}[1]{\overline{#1}}
    - \newcommand{\leg}[2]{\left(\frac{#1}{#2}\right)}
abstract: Chapter 24 on Rings of Polynomials
---

# A. Elementary Computation in Domains of Polynomials

## Q1

### $\mathbb{Z}[x]$

$$a(x) + b(x) = x^3 + 7x^2 + 4x + 1$$
$$a(x) - b(x) = -x^3 - 3x^2 + 2x + 1$$
\begin{align*}
a(x)b(x) &= 2x^5 + 10x^4 + 2x^3 + 3x^4 + 15x^3 + 3x^2 + x^3 + 5x^2 + x \\
&= 2x^5 + 13x^4 + 18x^3 + 8x^2 + x
\end{align*}

### $\mathbb{Z}_5[x]$

$$a(x) + b(x) = x^3 + 2x^2 + 4x + 1$$
$$a(x) - b(x) = 4x^3 + 2x^2 + 2x + 1$$
$$a(x)b(x) = 2x^5 + 3x^4 + 3x^3 + 3x^2 + x$$

### $\mathbb{Z}_6[x]$

$$a(x) + b(x) = x^3 + x^2 + 4x + 1$$
$$a(x) - b(x) = 5x^3 + 3x^2 + 2x + 1$$
$$a(x)b(x) = 2x^5 + x^4 + 2x^2 + x$$

### $\mathbb{Z}_7[x]$

$$a(x) + b(x) = x^3 + 4x + 1$$
$$a(x) - b(x) = 6x^3 + 4x^2 + 2x + 1$$
$$a(x)b(x) = 2x^5 + 6x^4 + 4x^3 + x^2 + x$$

## Q2

$$\mathbb{Z}: x^3 + x^2 + x + 1 = (x^2 + 3x + 1)(x - 2) + (5x - 5)$$
$$\mathbb{Z}_5: x^3 + x^2 + x + 1 = (x^2 + 3x + 2)(x + 3)$$

## Q3

$$\mathbb{Z}: x^3 + 2 = (\frac{x}{2} - \frac{3}{4})(2x^2 + 3x + 4) + (\frac{x}{4} + 5)$$
$$\mathbb{Z}_3: x^3 + 2 = (2x)(2x^2 + 3x + 4) + (-2x + 2)$$
$$\mathbb{Z}_5: x^3 + 2 = (3x + 3)(2x^2 + 3x + 4) + 4x$$

## Q4

### a

When $n = 1$, $x + 1$ is a factor of $x^n + 1$.

Assume $n = k$ is true
\begin{align*}
x^{k + 2} + 1 &= x^2 x^k \\
&= x^2(x^k + 1) + (1 - x^2) \\
&= x^2 (x^k + 1) (1 - x)(1 + x)
\end{align*}

Since $x + 1$ is a factor of $x^k + 1$, this means $x + 1$ is also a factor of $x^{k + 2}$.

### b

As before $n = 1$ is trivially true and we assume $n = k$ is true.

$$x^{k + 2} + x^{k + 1} + x^k + \cdots + x + 1 = x^2(x^k + \cdots + x + 1) + (x + 1)$$

Since $x + 1$ divides both terms, that means it is a divisor of the expression on the left.

## Q5

By induction assume $m = k$ is true, then
$$x^{k + 1} + 2 = x(x^k + 2) + (x + 2)$$
$(x + 2)$ divides both sides and so is a divisor of $x^{k + 1} + 2$ in $\mathbb{Z}_3[x]$.

Likewise for $\mathbb{Z}_n[x]$
\begin{align*}
x^{k + 1} + (n - 1) &= x(x^k + (n - 1)) + (x + (n - 1)) \\
&= x^{k + 1} + (n - 1)x + x + (n - 1) \\
&= x^{k + 1} + nx + (n - 1) \\
&= x^{k + 1} + (n - 1)
\end{align*}
and so $x + (n - 1) is a factor of $x^{k + 1} + (n - 1)$ in $\mathbb{Z}_n[x]$.

## Q6

\begin{align*}
(2x^2 + ax + b)(3x^2 + 4x + m) &= 6x^4 + 8x^3 + 2x^2 m + 3ax^3 + 4ax^2 + max + 3bx^2 + 4bx + mb \\
&= 6x^4 + 50
\end{align*}
grouping terms
$$6x^4 + (8 + 3a)x^3 + (2m + 4a + 3b)x^2 + (ma + 4b)x + mb = 6x^4 + 50$$

Writing out the roots, we have
$$8 + 3a = 0$$
$$2m + 4a + 3b = 0$$
$$ma + 4b = 0$$
$$mb = 50$$

The first equation has no solution since $3 \nmid a$ and so $6x^4 + 50$ cannot be factored into $3x^2 + 4x + m$.

## Q7

\begin{align*}
(x^3 + ax^2 + bx + c)(x^2 + 1) &= x^5 + x^3 + ax^4 + ax^2 + bx^3 + bx + cx^2 + c \\
&= x^5 + ax^4 + (1 + b)x^3 + (a + c)x^2 + bx + c \\
&= x^5 + 5x + 6
\end{align*}
Comparing terms, we have
\begin{align*}
a &\equiv 0 \mod n \\
1 + b &\equiv 0 \mod n \\
a + c &\equiv 0 \mod n \\
b &\equiv 5 \mod n \\
c &\equiv 6 \mod n \\
\implies 1 + 5 &\equiv 0 \mod n \\
\implies 6 &\equiv 0 \mod n
\end{align*}

$$n = 6, 2, 3$$

# B

## Q1

```python
>>> def foo(n):
...     print((n**8 + 1)%5, (n**3 + 1)%5)
... 
>>> for i in range(5):
...     foo(i)
... 
1 1
2 2
2 4
2 3
2 0
```

Both sides are not equal when $x = 2, 3, 4$.

## Q2

No this is impossible. If they are equal then their difference is 0.

## Q3

$$ 0x^2 + 0x + 0 $$
$$ 0x^2 + 0x + 1 $$
$$ 0x^2 + 0x + 2 $$
$$ \dots $$
$$ 0x^2 + 0x + 4 $$
$$ 0x^2 + 1x + 0 $$
$$ \dots $$
$$ 0x^2 + 4x + 0 $$
$$ 1x^2 + 0x + 0 $$
$$ \dots $$
$$ 4x^2 + 4x + 4 $$

There are $5^3$ polynomials in $\mathbb{Z}_5[x]$ of degree 2 or less. There are $5^2$ polynomials in $\mathbb{Z}_5[x]$ of degree 1 or 0.

Thus there are $5^3 - 5^2$ quadratic polynomials in $\mathbb{Z}_5[x]$.

Cubic:

$$ 0x^3 + 0x^2 + 0x + 0 $$
$$ \dots $$
$$ 0x^3 + 0x^2 + 0x + 4 $$
$$ 0x^3 + 0x^2 + 1x + 0 $$
$$ \dots $$
$$ 0x^3 + 0x^2 + 4x + 4 $$
$$ 0x^3 + 1x^2 + 0x + 0 $$
$$ \dots $$
$$ 0x^3 + 4x^2 + 4x + 4 $$
$$ 1x^3 + 0x^2 + 0x + 0 $$
$$ \dots $$
$$ 4x^3 + 4x^2 + 4x + 4 $$

Answer: $5^4 - 5^3$

There are $n^{m + 1} - n^m$ polynomials of degree $m$ in $\mathbb{Z}_n[x]$.

## Q4

$$(x + 1)^2 = x^2 + 2x + 1 = x^2 + 1 \text{ in } A[x] \implies \char A = 2$$
$$(x + 1)^4 = x^4 + 4x^3 + 6x^2 + 4x + 1 = x^4 + 1 \text{ in } A[x] \implies \char A = \gcd(4, 6) = 2$$
$$(x + 1)^6 = x^6 + 6x^5 + 15x^4 + 20x^3 + 15x^2 + 6x + 1 = x^6 + 2x^3 + 1 \text{ in } A[x] \implies \char A = \gcd(6, 15, 20 - 2) = 3$$

## Q5

$$(2x + 2)^3 = 8x^3 + 24x^2 + 24x + 8 = 0 \text{ in } \mathbb{Z}_8[x]$$
$$\implies  2x + 2 \text{ is a divisor of } 0$$

$$(1 - 4x)(1 + 4x) = 1 - 16x^2 = 1 \text{ in } \mathbb{Z}_8[x]$$
$$\implies 1 + 4x \text{ and } 1 - 4x \text{ are invertible elements}$$

## Q6

For any polynomial $b(x) \in A[x], \deg b(x) \geq 0$. If $\deg b(x) = 0$ then $xb(x) = 0$ because $b(x) = 0$. Otherwise $\deg [x \cdot b(x)] = \deg x + \deg b(x) = 1 + \deg b(x) \implies \deg [x \cdot b(x)] \geq 1$.

Since $x$ is in every non-zero polynomial domain, this means there are no polynomial fields.

## Q7

Take $a(x) = x \in A[x]$, then $\deg a(x) = 1$ and $\deg [(a(x))^2] = 2$. In fact $\deg[(a(x))^n] = n$ in any ring and so there is no polynomial with a nonzero term that multiplied by $x$ produces $0$.
$$x(b_0 + b_1 x + \cdots + b_m x^m)$$
where $b_m \neq 0$ in the ring, then
$$\deg [a(x) \cdot b(x)] = m + 1 \neq 0$$

## Q8

Idempotent: $(a(x))^2 = a(x)$
Nilpotent: $(a(x))^n = 0$ for some integer $n$.

Let $a(x) = x$, then $(a(x))^2 = x^2$, so $(a(x))^2 \neq a(x)$ and $a(x)$ is not idempotent.

Also $(a(x))^n = x^n \neq 0$ and so $a(x)$ is not nilpotent.

# C. Rings $A[x]$ Where $A$ Is Not an Integral Domain

## Q1

An integral domain is a commutative ring with unity having no divisors of 0.

Since $A[x]$ contains the elements from $A$, then if $A$ has zero divisors, so does $A[x]$ and hence $A[x]$ is not an integral domain.

## Q2

Degree 0: $2 \times 2 = 0$ in $\mathbb{Z}_4[x]$

Degree 1: $2x \cdot 2x = 0$

Degree 2: $2x^2 \cdot 2x^2 = 0$

## Q3

$5x^3(2x + 1) = 0$ in $\mathbb{Z}_10[x]$ lacks the cancellation property whereas the term $5x^3 = 0$ in $\mathbb{Z}_5[x]$ and disappears.

## Q4

Any polynomials where the coefficient of the leading term is a multiple of the field size.

$\mathbb{Z}_4[x]: (2x + 3)(2x + 1) = 3$

$\mathbb{Z}_6[x]: (3x + 1)(2x + 5) = 5x + 5$

$\mathbb{Z}_9[x]: (3x + 1)(3x + 4) = 6x + 4$

## Q5

$$a(x) = a_0 + a_1 x + \cdots + a_n x^n$$
$$b(x) = b_0 + b_1 x + \cdots + b_m x^m$$

$$\deg a(x) = n$$
$$\deg b(x) = m$$

$$a_n, b_m \in A : a_n \neq 0, b_m \neq 0, a_n b_m = 0$$

Thus the coefficient of x^{n + m} is 0 and so
$$\deg a(x) b(x) < \deg a(x) + \deg b(x)$$

## Q6

In an integral domain
$$\deg a(x)b(x) = \deg a(x) + \deg b(x)$$
Non-constant polynomials have a degree greater than one. Let $a(x)$ be such a polynomial, while $b(x)$ is a non-zero polynomial such that $\deg b(x) \geq 1$. Then $\deg a(x)b(x) > 1$, while the degree of 1 is 1. So there are no non-constant invertible polynomials in integral domains.

In $\mathbb{Z}_4[x], (2x + 1)^2 = 1$, so $(2x + 1)$ is invertible and so are all powers of $(2x + 1)^k$ since $(2x + 1)$ is its own inverse.

## Q7

### $\mathbb{Z}_9[x]$

$$(x + 3)(x + 6)$$
$$(2x + 3)(5x + 6)$$
$$(4x + 3)(7x + 6)$$
$$(5x + 3)(8x + 6)$$
$$(2x + 6)(5x + 3)$$
$$(4x + 6)(7x + 3)$$
$$(5x + 6)(8x + 3)$$

### $\mathbb{Z}_5[x]$

$$5 \mid (a + b) \qquad 5 \mid ab$$
but $\gcd(a, 5) = 1$ and $\gcd(b, 5) = 1$ since $5$ is prime. So there is only 1 factorization which is $x^2$.

## Q8

### $\mathbb{Z}_5[x]$

\begin{align*}
a + b &\equiv 1 \mod 5 \\
ab &\equiv 4 \mod 5
\end{align*}

\begin{align*}
2 + 4 &\equiv 1 \mod 5 \\
3 + 3 &\equiv 1 \mod 5 \\
2 \times 2 &\equiv 4 \mod 5 \\
3 \times 3 &\equiv 4 \mod 5
\end{align*}

\begin{align*}
(x + 3)^2 &= x^2 + x + 4 \\
[4(x + 3)]^2 &= 16x^2 + 96x + 144 \\
&= x^2 + x + 4 \\
&= (4x + 2)^2
\end{align*}

### $\mathbb{Z}_8[x]$

Any polynomial of the form $1 + 4x + 4x^2 + \cdots + 4x^n$ when squared will equal 1, because every coefficient apart from the constant and leading term is greater than or equal to 2, and $4\times 2 = 8 = 0$, and the leading term is $16x^{2n} = 0$. So there are infinite polynomial square roots in $\mathbb{Z}_8[x]$.

# D. Domains $A[x]$ Where $A$ Has Finite Characteristic

## Q1

Every coefficient in $A[x]$ is a member of $A$. For all $a(x), b(x) \in A[x], c(x) = a(x) + b(x)$ then $c_i = a_i + b_i$, and therefore the characteristic is preserved since $\underbrace{1_A + 1_A + \cdots + 1_A}_{\char A} = 0$.

## Q2

Consider the ring $\mathbb{Z}_n[x]$ of polynomials in one variable $x$ with coefficients in $\mathbb{Z}_n$. It is an infinite ring since $x^m \in \mathbb{Z}_n[x]$ for all positive integers $m$, and $x^{m_1} \neq x^{m_2}$ for $m_1 \neq m_2$. But the characteristic of $\mathbb{Z}_n[x]$ is clearly $n$.

## Q3

\begin{align*}
(x + 2)(x^{m - 1} + x^{m - 2} + \cdots + x^2 + x + 1) &= x(x^{m - 1} + x^{m - 2} + \cdots + x^2 + x + 1) + 2(x^{m - 1} + x^{m - 2} + \cdots + x^2 + x + 1) \\
&= x^m + (x^{m - 1} + x^{m - 2} + \cdots + x^3 + x^2 + x) + 2(x^{m - 1} + x^{m - 2} + \cdots + x^2 + x) + 2 \\
&= x^m + 2
\end{align*}

Likewise the above applies for $(p - 1)$ in any domain of characteristic $p$.

## Q4

By the cancellation property, the characteristic of every integral domain is prime, since if the characteristic was composite that would imply $rs = 0$ for some $r, s \in A$ which violates the zero divisor rule.

Thus the coefficients for all terms in the expansion $(x + c)^p$ except $x^p$ and $c^p$, by the binomial formula are equal to $\binom{p}{k} = \frac{p!}{k!(p - k)!}$. Since $p$ is prime and indivisible the coefficient becomes zero.
$$(x + c)^p = x^p + c^p$$

## Q5

They aren't the same since $x \notin A$, and $\forall a \in A$, $a = a^2$ but $x \neq x^2$.

## Q6

It is trivial to see that
\begin{align*}
[a_0 + (a_1x + \cdots + a_n x^n)]^p &= a_0^p + [a_1 x + (a_2 x^2 + \cdots + a_n x^n)]^p \\
&= a_0^p + a_1^p x^p + [a_2x^2 + (a_3 x^3 + \cdots + a_n x^n)]^p \\
&= a_0^p + a_1^p x_1^p + \cdots + a_n^p x^{np}
\end{align*}

# E. Subrings and Ideals in A[x]

## Q1

$B[x]$ contains all the polynomials with coefficients in $B$. Since $B$ is a subring of $A$, so $B[x]$ is a subring of $A[x]$.

## Q2

Likewise $B$ absorbs all products with $A$, and hence so does $B[x]$,

## Q3

Every coefficient $a_i$ with odd $i$ equal to zero, means the polynomial only has non-zero coefficients for even powers.

When adding polynomials, we add the coefficients. So the odd numbered powers remain zero, and even powers remain non-zero.

For multiplying two polynomials $a(x)b(x)$, the corresponding powers of each term are added together, $a_i b_j x^{i + j}$. Since both $i$ and $j$ are even, so is the resulting term and hence the result of $a(x)b(x)$ remains inside the set $S$ making it a subring.

The above statement does not apply when talking about odd non-zero coefficients, since multiplying two odd terms might result in an even power, for example $c(x) = a(x) b(x)$, $a_3 b_5 x^{3 + 5}$.

## Q4

Let $b(x) \in A[x]$ and $a(x) \in J$, then the constant term in $b(x)$ is $b_0$. Since $b(x) a(x) = b_0 a(x) + b_1 x a(x) + \cdots + b_m x^n a(x)$, and the powers of all terms in $a(x)$ are $\geq 1$, so $b_0 a(x)$ has no constant term. So $\forall a(x) \in J$ absorbs products from $A[x]$ and is an ideal.

## Q5

Let $a(x) = a_0 + a_1x + \cdots + a_n x^n \in J$ and $b(x) = b_0 + b_1x + \cdots + b_m x^m \in A[x]$. Then $a(x)b(x) = a_0 (b_0 + b_1x + \cdots + b_m x^m) + a_1x (b_0 + b_1x + \cdots + b_m x^m) + \cdots + a_n x^n (b_0 + b_1x + \cdots + b_m x^m)$. Then it can be seen plainly that the sum of cofficients for the result is $(a_0 + a_1 + \cdots + a_n)(b_0 + b_1 + \cdots + b_m) = 0$. Therefore $J$ is an ideal of $A[x]$.

## Q6

Since $A$ is an integral domain, there are no divisors of zero. Therefore the values cannot be made to equal 0 unless one of the terms is zero. In the case of Q4, the polynomial is an ideal in $J$ with a zero constant coefficient and in Q5, the polynomial can be factorized into a polynomial where one of the terms has coefficients that sum to zero.

# F. Homomorphisms of Domains of Polynomials

## Q1

$$a(x) = a_0 + a_1 x + \cdots + a_n x^n$$
$$b(x) = b_0 + b_1 x + \cdots + b_m x^m$$

$$h(a(x) + b(x)) = h((a_0 + b_0) + \cdots) = a_0 + b_0 = h(a(x)) + h(b(x))$$
$$h(a(x)b(x)) = h(a_0 b_0 + \cdots) = a_0 b_0 = h(a(x))h(b(x))$$

## Q2

$$\forall a(x) \in A[x], h(x \cdot a(x)) = h(x(a_0 + \cdots + a_n x^n)) = h(a_0 x + \cdots + a_n x^{n + 1}) = 0$$
$$\implies \ker h = \{ x \cdot a(x) : a(x) \in A[x] \} = \langle x \rangle$$

By the definition of a principal ideal, let $x$ remain fixed as it is multiplied by elements from $A[x]$.

## Q3

$$h : A[x] \rightarrow A, \ker h = \langle x \rangle \implies A[x] / \langle x \rangle \cong A$$

## Q4

$$g(a(x)) = g(a_0 + \cdots + a_n x^n) = a_0 + \cdots + a_n$$

\begin{align*}
g(a(x) + b(x)) &= g(a_0 + a_1 x + \cdots + a_m x^m + \cdots + a_n x^n + b_0 + b_1 x + \cdots + b_m x^m) \\
&= (a_0 + b_0) + (a_1 + b_1) + \cdots + (a_m + b_m) + \cdots + a_n \\
&= g(a(x)) + g(b(x))
\end{align*}

\begin{align*}
g(a(x)b(x)) &= g(a_0 b(x) + a_n x^n b(x)) \\
&= g(a_0 b_0 + \cdots + a_0 b_m x^m + \cdots + a_n b_0 x^n + \cdots + a_n b_m x^{n + m}) \\
& = a_0 b_0 + \cdots + a_0 b_m + \cdots + a_n b_m = g(a(x)) g(b(x))
\end{align*}

Let $a \in A$, then $a(x) \in J + a$, where $J$ is the ideal of $g$ (coefficients that sum to zero). Thus every value in $A$ is an image of an element in $A[x]$ and so $h$ is surjective.

The kernel of $g$ is described in 24E5: let $J$ consist of all the polynomials $a_0 + a_1 x + \cdots + a_n x^n$ in $A[x]$ such that $a_0 + a_1 + \cdots + a_n = 0$.

## Q5

\begin{align*}
h(a(x) + b(x)) &= (a_0 + b_0) + (a_1 + b_1) cx + (a_2 + b_2)c^2 x^2 + \cdots + (a_n + b_n) c^n x^n \\
&= (a_0 + a_1 cx + a_2 c^2 x^2 + \cdots + a_n c^n x^n) + (b_0 + b_1 cx + b_2 c^2 x^2 + \cdots + b_n c^n x^n) \\
&= h(a(x)) + h(b(x))
\end{align*}

\begin{align*}
h(a(x)b(x)) &= a_0 b_0 + (a_0 b_1 + a_1 b_0) cx + (a_0 b_2 + a_1 b_1 + a_0 b_2) c^2 x^2 + \cdots + \sum_{i + j = n} a_i b_j c^n x^n \\
&= h(a(x))h(b(x))
\end{align*}

Since $A$ is an integral domain and there are no zero divisors, then $\ker h = \{ 0 \}$.

## Q6

Any polynomial $a(x) = a_0 + a_1 x + \cdots + a_n x^n$ can be produced by $h$ iff $c$ is invertible by setting the input to $a_0 + c^{-1} a_1 x + \cdots + c^{-n} a_n x^n$. Then the output of $h$ on this value will produce $a(x)$. Thus $h$ is an automorphism in this case.

# G. Homomorphisms of Polynomial Domains Induced by a Homomorphism of the Ring of Coefficients

## Q1

$$\bar{h}(a_0 + a_1 x + \cdots + a_n x^n) = h(a_0) + h(a_1)x + \cdots + h(a_n)x^n$$

\begin{align*}
\bar{h}(a(x) + b(x)) &= \bar{h}((a_0 + b_0) + (a_1 + b_1)x + \cdots + (a_n + b_n) x^n) \\
&= h(a_0 + b_0) + h(a_1 + b_1) x + \cdots + h(a_n + b_n) x^n \\
&= (h(a_0) + h(b_0)) + (h(a_1) + h(b_1)) x + \cdots + (h(a_n) + h(b_n)) x^n \\
&= \bar{h}(a(x)) + \bar{h}(b(x))
\end{align*}

\begin{align*}
\bar{h}(a(x)b(x)) &= \bar{h}(a_0 b_0 + a_0 b_1 x + \cdots + a_n b_n x^{2n}) = h(a_0 b_0) + h(a_0 b_1) x + \cdots + h(a_n b_n) x^{2n} \\
&= h(a_0) h(b_0) + h(a_0) h(b_1) x + \cdots + h(a_n) h(b_n) x^{2n} \\
&= \bar{h}(a(x))\bar{h}(b(x))
\end{align*}

## Q2

$$\forall a_i : 0 \leq i \leq n, a_i \in \ker h$$
$$a(x) = a_0 + \cdots + a_n x^n$$

## Q3

If $h$ is surjective, then every element of $B$ is of the form $h(a)$ for some $a$ in $A$. Thus, any polynomial with coefficients in $B$ is of the form $h(a_0) + h(a_1)x + \cdots + h(a_n)x^n = \bar{h}(a_0 + a_1 x + \cdots + a_n x^n)$.

## Q4

Every coefficient of $A[x]$ maps to a distinct coefficient in $B[x]$ because $h$ is an injective function.

## Q5

$$b(x) = q(x)a(x)$$
$$\bar{h}(b(x)) = \bar{h}(q(x))\bar{h}(a(x))$$

## Q6

Every coefficient $a_i = qn$ and so $h(a_i) = 0$ because $n \mid a_i$. Thus $\bar{h}(a(x)) = 0$.

## Q7

$\mathbb{Z}_n$ where $n$ is prime, means the domain of $\bar{h}$ is an integral domain.
$$\bar{h} : \mathbb{Z}[x] \underset{\ker \bar{h}}{\relbar\joinrel\twoheadrightarrow} \mathbb{Z}_n[x]$$

From 19F2, $J$ is a prime ideal iff $A/J$ is an integral domain. So in our case this means $\ker \bar{h}$ is a prime ideal.

An ideal $J$ of a commutative ring is said to be a prime ideal if for any two elements $a$ and $b$ in the ring,
$$\text{If } ab \in J \text{ then } a \in J \text{ or } b \in J$$

$$a(x)b(x) \in \ker \bar{h} \implies a(x) \text{ or } b(x) \in \ker \bar{h}$$

# H. Polynomials in Several Variables

## Q1

*Prove $A$ is an integral domain $\implies A[x]$ is an integral domain.$

Given any $A_i[x_{i + 1}]$ is an integral domain, we know that the leading term $a_k \neq 0$ (which includes the other non-zero $x$ values), multiplied by another $b_l \neq 0$, and so $a_k b_l \neq 0$ and therefore $A_i[x_{i + 1}]$ has a non-zero coefficient.

## Q2

Degree of $p(x, y)$ is the greatest $n$ such that the coefficient $a_n$ is non-zero for the powers $x^i y^j$ such that $i + j = n$.

$$0, 1, 2$$
$$x, x + 1, x + 2$$
$$2x, 2x + 1, 2x + 2$$
$$x^2, x^2 + 1, x^2 + 2$$
$$x^2 + x, x^2 + x + 1, x^2 + x + 2$$
$$\cdots$$
$$2x^3 + 2x^2 + 2x, 2x^3 + 2x^2 + 2x + 1, 2x^3 + 2x^2 + 2x + 2$$

## Q3

\begin{align*}
a(x, y) + b(x, y) &= (a_{0,0} + b_{0, 0}) + (a_{1, 0} + b_{1, 0})x + \cdots + (a_{n, 0} + b_{n, 0}) x^n \\
&\quad + (a_{0, 1} + b_{0, 1}) y + (a_{1, 1} + b_{1, 1}) xy + \cdots + (a_{n, 1} + b_{n, 1}) x^n y + \cdots \\
&\quad + (a_{0, n} + b_{0, n}) y^n + (a_{1, n} + b_{1, n})xy^n + \cdots + (a_{n, n} + b_{n, n})x^n y^n \\
&= \sum_{i = 0}^n \sum_{j = 0}^n (a_{i,j} + b_{i, j}) x^i y^j
\end{align*}

\begin{align*}
a(x, y) b(x, y) &= a_{0, 0} b_{0, 0} + (a_{0, 0} b_{1, 0} + a_{0, 1} b_{0, 0}) x \\
&\quad + (a_{0, 0} b_{2, 0} + a_{1, 0} b_{1, 0} + a_{2, 0} b_{0, 0}) x^2 + \cdots + a_{n, 0} b_{n, 0} x^{2n} \\
&\quad + (a_{0, 1} b_{1, 0} + a_{1, 1} b_{0, 0} + a_{0, 0} b_{1, 1} + a_{1, 0} b_{0, 1}) xy \\
&\quad + (a_{0, 1} b_{2, 0} + a_{0, 0} b_{2, 1} + a_{1, 1} b_{1, 0} + a_{1, 0} b_{1, 1} + a_{2, 1} b_{0, 0} + a_{2, 0} b_{0, 1}) x^2 y \\
&\quad + \cdots + a_{n, n} b_{n, n} x^{2n} y^{2n}
&= (c_{0, 0} + c_{1, 0} x + \cdots + c_{2n, 0} x^{2n}) \\
&\quad + c_{0, 1} y + c_{1, 1} xy + \cdots + c_{2n, 1} x^{2n} y \\
&\quad + \cdots + c_{0, 2n} y^{2n} + c_{1, 2n} xy^{2n} + \cdots + c_{2n, 2n} x^{2n} y^{2n} \\
&= \sum_{i = 0}^{2n} \sum_{j = 0}^{2n} c_{i,j} x^i y^j
\end{align*}

$$c_{k, l} = \sum_{i_x + j_x = k, \; i_y + j_y = l}{a_{i_x, i_y} b_{j_x, j_y}}$$

## Q4

If there are two or more terms with the same degree, we ignore them since they do not cancel. For example $xy$ and $y^2$.

The coefficient for the leading term is of the form
$$a_{m, s} b_{n, t} \text{ for } a(x, y) b(x, y)$$

Thus $\deg a(x, y) b(x, y) = (m + n) + (s + t)$
$$\deg a(x, y) b(x, y) = \deg a(x, y) + \deg b(x, y)$$

# I. Fields of Polynomial Quotients

## Q1

$A$ is a finite integral domain means it is a field with $\char(A)$ for $1_A$. The unity for $A(x)$ is $[1_A, 1_A]$ and $[a, b] + [c, d] = [ad + bc, bd]$.
$$[1_A, 1_A] + [1_A, 1_A] = [2_A, 1_A]$$
$$[k_A, 1_A] + [1_A, 1_A] = [k_A + 1_A, 1_A]$$
\begin{align*}
\underbrace{[1_A, 1_A] + \cdots + [1_A, 1_A]}_{\char(A)} &= [\char(A), 1_A] \\
&= [0_A, 1_A]
\end{align*}

## Q2

$\mathbb{Z}_p$ is a finite field with characteristic $p$. Therefore the field of quotients $\mathbb{Z}_p(x)$ will have characteristic $p$ yet it is infinite because terms have any positive integer value (and indeed negative since $\mathbb{Z}_p$ has inverses because it is a field).

## Q3

\begin{align*}
\bar{h}\left(\frac{a(x)}{s(x)}\right) &= \bar{h}\left(\frac{a_0 + \cdots + a_n x^n}{s_0 + \cdots + s_n x^n}\right) \\
&= \frac{h(a_0) + \cdots + h(a_n) x^n}{h(s_0) + \cdots + h(s_n)x^n}
\end{align*}

Because $h$ is isomorphic, each element of $B(x)$ is the image of no more than one element of $A(x)$, so $\bar{h}$ is injective.

Likewise every element of $B(x)$ is the image of an element in $A(x)$, so $\bar{h}$ is surjective.

$\therefore \bar{h}$ is an isomorphism.

# J. Division Algorithm: Uniqueness of Quotient and Remainder

*In the division algorithm, prove that $q(x)$ and $r(x)$ are uniquely determined. [HINT: Suppose $a(x) =
b(x)q_1 (x) + r_1 (x) = b(x)q_2 (x) + r_2 (x)$, and subtract these two expressions, which are both equal to $a(x)$.]*

$$ 0 = b(x)(q_1(x) - q_2(x)) + (r_1(x) - r_2(x)) $$

Assume $\deg b(x) > 0$.

If $q_1(x) \neq q_2(x)$, then $\deg [q_1(x) - q_2(x)] > 0$ so $\deg [b(x)(q_1(x) - q_2(x)] > 0$.

But the entire expression is 0 and so its degree is zero. Hence $b(x)(q_1(x) - q_2(x))$ cannot have a degree higher than 0 so the term can only equal 0, which means $q_1(x) = q_2(x)$ since $b(x) \neq 0$.

$$\implies r_1(x) - r_2(x) = 0$$
