---
title: Abstract Algebra by Pinter, Chapter 25
author: Amir Taaki
header-includes: |
    - \usepackage{mathrsfs}
    - \usepackage{mathtools}
    - \usepackage{extpfeil}
    - \DeclareMathOperator\ker{ker}
    - \DeclareMathOperator\ord{ord}
    - \DeclareMathOperator\gcd{gcd}
    - \DeclareMathOperator\lcm{lcm}
    - \DeclareMathOperator\char{char}
    - \DeclareMathOperator\max{max}
    - \DeclareMathOperator\ran{ran}
    - \DeclareMathOperator\deg{deg}
    - \newcommand{\mod}[1]{\ (\mathrm{mod}\ #1)}
    - \newcommand{\repr}[1]{\overline{#1}}
    - \newcommand{\leg}[2]{\left(\frac{#1}{#2}\right)}
abstract: Chapter 24 on Factoring Polynomials
---

# A. Examples of Factoring into Irreducible Factors

## Q1

$\mathbb{Q}: x^4 - 4 = (x^2 - 2)(x^2 + 2)$

$\mathbb{R}: x^4 - 4 = (x - \sqrt{2})(x + \sqrt{2})(x^2 + 2)$

$\mathbb{C}: x^4 - 4 = (x - \sqrt{2})(x + \sqrt{2})(x - \sqrt{2}i)(x + \sqrt{2}i)$

## Q2

Factor $x^6 - 16$

$\mathbb{Q}: (x^3 - 4)(x^3 + 4)$

$\mathbb{R}: (x^3 - (\sqrt[3]{4})^3)(x^3 + (\sqrt[3]{4})^3) = (x - \sqrt[3]{4})(x^2 + \sqrt[3]{4} x + (\sqrt[3]{4})^2) (x + \sqrt[3]{4})(x^2 - \sqrt[3]{4} x + (\sqrt[3]{4})^2)$

(using the sum and differences of cubes formulas: $a^3 + b^3 = (a + b)(a^2 - ab + b^2)$ and $a^3 - b^3 = (a - b)(a^2 + ab + b^2)$.)

Using the quadratic formula to find the roots, for $\mathbb{C}$ and setting $b = \sqrt[3]{4}$ we get:

$$(x^6 - 16) = (x - b)(x^2 + b x + b^2) (x + b)(x^2 - b x + b^2)$$
$$a = 1, b = \sqrt[3]{4}, c = b^2 = (\sqrt[3]{4})^2$$
\begin{align*}
x &= \frac{-b \pm \sqrt{b^2 - 4ac}}{2a} \\
  &= \frac{-b \pm \sqrt{b^2 - 4b^2}}{2} \\
  &= \frac{-b \pm b \sqrt{-3}}{2} \\
  &= \frac{-b - b \sqrt{3}i}{2}, \frac{-b + b \sqrt{3}i}{2} \\
\end{align*}

And so therefore the roots for $(x^2 + bx + b^2)$ are:

\begin{align*}
(x^2 + bx + b^2) &= (x - [\frac{-b - b \sqrt{3}i}{2}])(x - [\frac{-b + b \sqrt{3}i}{2}]) \\
(x^2 + \sqrt[3]{4}x + (\sqrt[3]{4})^2) &=  (x - [\frac{-\sqrt[3]{4} - \sqrt[3]{4} \sqrt{3}i}{2}])(x - [\frac{-\sqrt[3]{4} + \sqrt[3]{4} \sqrt{3}i}{2}]) \\
 &=  \left(x + \frac{\sqrt[3]{4}}{2} - \frac{\sqrt[3]{4}}{2} \sqrt{3}i\right)\left(x + \frac{\sqrt[3]{4}}{2} + \frac{\sqrt[3]{4}}{2} \sqrt{3}i\right) \\
\end{align*}
Likewise
$$(x^2 - \sqrt[3]{4}x + (\sqrt[3]{4})^2) =
   \left(x - \frac{\sqrt[3]{4}}{2} - \frac{\sqrt[3]{4}}{2} \sqrt{3}i\right)\left(x - \frac{\sqrt[3]{4}}{2} + \frac{\sqrt[3]{4}}{2} \sqrt{3}i\right)
$$
Thus
$$(x^6 - 16) =
   (x - \sqrt[3]{4})
   \left(x + \frac{\sqrt[3]{4}}{2} - \frac{\sqrt[3]{4}}{2} \sqrt{3}i\right)\left(x + \frac{\sqrt[3]{4}}{2} + \frac{\sqrt[3]{4}}{2} \sqrt{3}i\right)
   (x + \sqrt[3]{4})
   \left(x - \frac{\sqrt[3]{4}}{2} - \frac{\sqrt[3]{4}}{2} \sqrt{3}i\right)\left(x - \frac{\sqrt[3]{4}}{2} + \frac{\sqrt[3]{4}}{2} \sqrt{3}i\right)
   $$

