---
title: Abstract Algebra by Pinter, Chapter 26
author: Amir Taaki
header-includes: |
    - \usepackage{mathrsfs}
    - \usepackage{mathtools}
    - \usepackage{extpfeil}
    - \DeclareMathOperator\ker{ker}
    - \DeclareMathOperator\ord{ord}
    - \DeclareMathOperator\gcd{gcd}
    - \DeclareMathOperator\lcm{lcm}
    - \DeclareMathOperator\char{char}
    - \DeclareMathOperator\max{max}
    - \DeclareMathOperator\ran{ran}
    - \DeclareMathOperator\deg{deg}
    - \newcommand{\mod}[1]{\ (\mathrm{mod}\ #1)}
    - \newcommand{\repr}[1]{\overline{#1}}
    - \newcommand{\leg}[2]{\left(\frac{#1}{#2}\right)}
abstract: Chapter 26 on Substitution in Polynomials
---

# A. Finding Roots of Polynomials over Finite Fields

## Q1

### $f(x) = x^3 + x^2 + x + 1$

$f(4) = 0 \implies (x + 1)$ is a factor.

$f(x) / (x + 1) = x^2 + 1$, and $x^2 + 1 = (x + 3)(x - 3)$ because $(2)^2 + 1 = 0$, so $f(x) = (x + 1)(x + 3)(x - 3)$.

### $f(x) = 3x^4 + x^2 + 1$

$f(1) = 0 \implies (x + 4)$ is a factor.

$f(4) = 0 \implies (x + 1)$ is a factor.

$(x + 4)(x + 1) = x^2 + 4$. And $f(x) / (x^2 + 4) = 3x^2 + 4$

$f(x) = (x + 4)(x + 1)(3x^2 + 4)$

### $f(x) = x^5 + 1$

$(x + 1)$ is a factor.
\begin{align*}
(x + 1)^5 &= x^5 + 5x^4 + 10x^3 + 10x^2 + 5x + 1 \\
&= x^5 + 1
\end{align*}

### $f(x) = x^4 + 1$

No roots

### $f(x) = x^4 + 4$

$f(1), f(2), f(3), f(4) = 0$

$x^4 + 4 = (x + 1)(x + 2)(x + 3)(x + 4)$. That is all values of $\mathbb{Z}_5[x]$ where $a \neq 0$.

## Q2

### $a(x) = x^{100} - 1$

$\phi(7) = 6$ and so $x^{100} \equiv (x^6)^{16} x^4 \equiv x^4 \mod 7$ because $x^6 = 1$. This is true for all $a \in \mathbb{Z}_7$ so any root in $x^{100} - 1$ must also be in $x^4 - 1$.

$f(1), f(6) = 0$ so these are the roots.

### $a(x) = 3x^{98} + x^{19} + 3$

$\forall a \in \mathbb{Z}_7[x], 3x^{98} + x^{19} + 3 = 3x^2 + x + 3$. The only root is 1.

### $a(x) = 2x^{74} - x^{55} + 2x + 6$

$a(x) = 2x^2 + x + 6$. Roots are 4 and 6.

## Q3

$$3x^3 - 5 + 2x - x^2$$

$$5 + 6x^5 - 2x^3$$

$$3x - x + 3x - x = 4x$$

## Q4

Power act like an additive group modulo $\phi(p) = p - 1$, so any $x^{\phi(p)q + r}$ where $r < \phi(p)$ can be reduced to $x^r$.

# B. Finding Roots of Polynomials over $\mathbb{Q}$

## Q1

### $9x^3 + 18x^2 - 4x - 8$

$a_0 = -8$ and $a_n = 9$.
$$s = \pm 1, \pm 8, \pm 2, \pm 4$$
$$t = \pm 1, \pm 9, \pm 3$$
Possible roots are $\pm 1, \pm 2, \pm 4, \pm 8, \pm 1/9, \pm 1/3, \pm 8/9, \pm 8/3, \pm 2/9, \pm 2/3, \pm 4/9, \pm 4/3$. Substituting in we find roots for 2, $\pm 2/3$.
$$9x^3 + 18x^2 - 4x - 8 = 9(x - 2/3)(x + 2/3)(x + 2)$$

### $4x^3 - 3x^2 - 8x + 6$

$a_0 = 6$ and $a_n = 4$.
$$s = \pm 1, \pm 6, \pm 2, \pm 3$$
$$t = \pm 1, \pm 4, \pm 2$$
Possible roots are $\pm 1, \pm 6, \pm 2, \pm 3, \pm 3/2, \pm 1/2, \pm 3/4$. Substituting in we find a root for $3/4$. Dividing $a(x)$ by $(x - 3/4)$ in sage, we get $4x^2 - 8$ as the remaining term.

$$4x^3 - 3x^2 - 8x + 6 = 4(x - 3/4)(x^2 - 2)$$

### $2x^4 + 3x^3 - 8x - 12$

$a_0 = -12$ and $a_n = 2$
$$s = \pm 1, \pm 12, \pm 3, \pm 2, \pm 4, \pm 6$$
$$t = \pm 1, \pm 2$$
Possible roots: $\pm 1, \pm 12, \pm 3, \pm 2, \pm 4, \pm 6, \pm 3/2$. Root is $-3/2$. Dividing by $(x + 3/2)$, we get $(2x^3 - 8)$ as the remaining term.

$$2x^4 + 3x^3 - 8x - 12 = 2(x + 3/2)(x^3 - 4)$$

### $6x^4 - 7x^3 + 8x^2 - 7x + 2$

$a_0 = 2$ and $a_n = 6$
$$s = \pm 1, \pm 2$$
$$t = \pm 1, \pm 6, \pm 2, \pm 3$$
Possible roots: $\pm 1, \pm 2, \pm 1/6, \pm 1/2, \pm 1/3, \pm 2/3$. Roots: $1/2, 2/3$. Dividing by $(x - 1/2)(x - 2/3)$, we get $6(x^2 + 1)$ as the remaining term.

$$6x^4 - 7x^3 + 8x^2 - 7x + 2 = 6(x - 1/2)(x - 2/3)(x^2 + 1)$$

## Q2

### $9x^3 + 18x^2 - 4x - 8$

$$9x^3 + 18x^2 - 4x - 8 = 9(x - 2/3)(x + 2/3)(x + 2)$$

#### $\mathbb{R}[x]$

Unchanged from above.

#### $\mathbb{C}[x]$

Unchanged from above. Every factor is of degree 1.

### $4x^3 - 3x^2 - 8x + 6$

$$4x^3 - 3x^2 - 8x + 6 = 4(x - 3/4)(x^2 - 2)$$

#### $\mathbb{R}[x]$

$$(x^2 - 2) = (x - \sqrt{2})(x + \sqrt{2})$$
$$4x^3 - 3x^2 - 8x + 6 = 4(x - 3/4)(x - \sqrt{2})(x + \sqrt{2})$$

#### $\mathbb{C}[x]$

Unchanged from above

### $2x^4 + 3x^3 - 8x - 12$

$$2x^4 + 3x^3 - 8x - 12 = 2(x + 3/2)(x^3 - 4)$$

#### $\mathbb{R}[x]$

$$(x^3 - 4) = (x - \sqrt[3]{4})(x^2 + \sqrt[3]{4}x + (\sqrt[3]{4})^2)$$
$$2x^4 + 3x^3 - 8x - 12 = 2(x + 3/2)(x - \sqrt[3]{4})(x^2 + \sqrt[3]{4}x + (\sqrt[3]{4})^2)$$

#### $\mathbb{C}[x]$

Let $A = \sqrt[3]{4}$
$$x^2 + Ax + A^2 = 0$$
$$(x + A/2)^2 - (A/2)^2 + A^2 = (x + A/2)^2 + (A/2)^2 = 0$$
$$\implies x = \sqrt{-(A/2)^2} - A/2 = \pm iA/2 - A/2$$
\begin{align*}
\implies x^2 + Ax + A^2 &= (x - (\pm iA/2 - A/2)) \\
&= (x + A/2 + iA/2)(x + A/2 - iA/2)
\end{align*}
$$2x^4 + 3x^3 - 8x - 12 = 2(x + 3/2)(x - A)(x + A/2 + iA/2)(x + A/2 - iA/2)$$

### $6x^4 - 7x^3 + 8x^2 - 7x + 2$

$$6x^4 - 7x^3 + 8x^2 - 7x + 2 = 6(x - 1/2)(x - 2/3)(x^2 + 1)$$

#### $\mathbb{R}[x]$

Same as above.

#### $\mathbb{C}[x]$

$$(x^2 + 1) = (x - i)(x + i)$$
$$6x^4 - 7x^3 + 8x^2 - 7x + 2 = 6(x - 1/2)(x - 2/3)(x - i)(x + i)$$

## Q3

$$18x^3 + 27x^2 - 8x - 12$$
$$2x^3 - x^2 - 2x + 1$$
$$3x^3 + x^2 - 3x - 1$$

## Q4

### $18x^3 + 27x^2 - 8x - 12$

$$a_0 = -12, a_n = 18$$
Factors of $a_0: \pm 1, \pm 2, \pm 3, \pm 4, \pm 6, \pm 12$

Factors of $a_n: \pm 1, \pm 2, \pm 3, \pm 6, \pm 9, \pm 18$

```py
a = lambda x: 18*x**3 + 27*x**2 - 8*x - 12

for s in [1, 2, 3, 4, 6, 12]:
    for t in [1, 2, 3, 6, 9, 18]:
        st = s/t
        if abs(a(st)) < 0.001:
            print("+", s, t)
        if abs(a(-st)) < 0.001:
            print("-", s, t)
```

Output:

```
+ 2 3
- 2 3
- 3 2
+ 4 6
- 4 6
+ 6 9
- 6 9
+ 12 18
- 12 18
```

Roots: $\pm 2/3, -3/2$

$(x - 2/3)(x + 2/3)(x + 3/2)$

### $2x^3 - x^2 - 2x + 1$

$$a_0 = 1, a_n = 2$$
Factors of $a_0: \pm 1$

Factors of $a_n: \pm 1, \pm 2$

Roots: $\pm 1, 1/2$

$$\frac{1}{2}(x + 1)(x - 1)(x - 1/2)$$

### $3x^3 + x^2 - 3x - 1$

$$a_0 = -1, a_n = 3$$
Factors of $a_0: \pm 1$

Factors of $a_n: \pm 1, \pm 3$

Roots: $\pm 1, -1/3$

$$\sqrt{3}(x + 1)(x - 1)(x + 1/3)$$

## Q5

$$2x^4 + 3x^2 - 2 = (2x^2 + 1)(x^2 - 2)$$

So there are no rational roots.

# C. Short Questions Relating to Roots

## Q1

Let $a(x) = p(x) - p(c)$, then $a(c) = 0 \implies (x - c) \mid [p(x) - p(x)]$ and so $p(x) - p(c) = q(x)(x - c)$ or $p(x) = q(x)(x - c) + p(c)$. $\deg p(c) = 0$ and $\deg (x - c) = 1$.

## Q2

\begin{align*}
p(x) - p(c) &= a_1(x - c) + \cdots + a_n(x^n - c^n) \\
&= q(x)(x - c) + r(x)
\end{align*}
$$\deg r(x) < \deg (x - c) \implies r(x) = r \geq 0$$
$$p(c) - p(c) = 0 = q(x)(c - c) + r = 0 + r = r$$
Thus $r = 0$ and $(x - c) \mid (p(x) - p(c))$.

## Q3

$a(x)$ and $b(x)$ are associates if $a(x) \mid b(x)$ and $b(x) \mid a(x) \iff$ they are constant multiples of each other. So $a(x) = db(x)$, and $b(c) = 0 \implies a(x) = db(c) = d \cdot 0 = 0$.

## Q4

$a(x) = (x - c)^m$ and $b(x) = (x - c)^n$ both have the same roots but differ by non-constant factors and so are not associates.

## Q5

$a(x)$ has $n$ roots $c_1, \dots, c_n \in F$
$$\implies a(x) = q(x)[(x - c_1) \cdots (x - c_n)]$$
but $\deg [(x - c_1)\cdots (x - c_n)] = n = \deg a(x)$ and $a(x)$ is monic, and so is $(x - c_1) \dots (x - c_n) = x^n + \cdots + (-c_1)\cdots(-c_n) \implies q(x) = 1$
and so
$$a(x) = (x - c_1) \cdots (x - c_n)$$

## Q6

$$a(c) = b(c) \implies a(c) - b(c) = 0$$
Let $\deg [a(x) - b(x)] = m < n$, then $a(x) - b(x)$ can be factored in at most $m$ ways $(x - c_1)\cdots (x - c_m)$ but there exists a $c$ such that $c \neq c_i$ for all $m$ values, yet
$$a(c) - b(c) = 0 = k(c - c_1) \cdots (c - c_m)$$
by the fact $F$ is a field, then $F[x]$ is an integral domain and has no zero divisors. This means $k = 0$ since all the other terms are nonzero.
$$a(x) - b(x) = 0$$
$$a(x) = b(x)$$

## Q7

In $\mathbb{Z}_5, 2 \nmid 1$ and $2^2 \nmid 2$, so by Eisenstein's irreducibility criterion, any polynomial of the form
$$2 + \cdots + x^n$$
is irreducible. There are an infinite number of these polynomials.

## Q8

$$x(x - 1) = 0$$
$$\mathbb{Z}_{10}: 0, 1, 5, 6$$
$$\mathbb{Z}_{11}: 0, 1$$
there are no divisors of zero in $\mathbb{Z}_11$.

