---
title: Abstract Algebra by Pinter, Chapter 29
author: Amir Taaki
header-includes: |
    - \usepackage{mathrsfs}
    - \usepackage{mathtools}
    - \usepackage{extpfeil}
    - \DeclareMathOperator\ker{ker}
    - \DeclareMathOperator\ord{ord}
    - \DeclareMathOperator\gcd{gcd}
    - \DeclareMathOperator\lcm{lcm}
    - \DeclareMathOperator\char{char}
    - \DeclareMathOperator\max{max}
    - \DeclareMathOperator\ran{ran}
    - \DeclareMathOperator\deg{deg}
    - \DeclareMathOperator\dim{dim}
    - \newcommand{\mod}[1]{\ (\mathrm{mod}\ #1)}
    - \newcommand{\repr}[1]{\overline{#1}}
    - \newcommand{\leg}[2]{\left(\frac{#1}{#2}\right)}
    - \let\vec\mathbf
abstract: Chapter 29 on Degress of Field Extensions
---

# A. Examples of Finite Extensions

## Q1

$x^2 + 2$ has root $i\sqrt{s}$

$$[\mathbb{Q}(i\sqrt{2}) : \mathbb{Q}] = 2$$
$$\mathbb{Q}(i\sqrt{2}) = \{ a + bi \sqrt{2} \}$$

## Q2

$$x = 2 + 3i$$
$$(x - 2)^2 = -9$$
$$x^2 - 4x + 13 = 0$$
$$\{a, bi\}$$

## Q3

$$a = \sqrt{1 + \sqrt[3]{2}}$$
$$a^2 + 1 = \sqrt[3]{2}$$
$$a^2 + 1 \in \mathbb{Q}(a) \implies \sqrt[3]{2} \in \mathbb{Q}(a)$$
$$x = \sqrt[3]{2}$$
$$\therefore x^3 - 2 = 0$$
$$[\mathbb{Q}(\sqrt[3]{2}):\mathbb{Q}] = 3$$
Basis for $\mathbb{Q}(\sqrt[3]{2})$ is $\{ 1, 2^{\frac{1}{3}}, 2^{\frac{1}{3}}\}$
$$a^2 + (1 - \sqrt[3]{2}) = 0$$
$$\sqrt[3]{2} \in \mathbb{Q}(a) \implies \mathbb{Q}(a) = \mathbb{Q}(a, \sqrt[3]{2})$$
$$[\mathbb{Q}(a): \mathbb{Q}(\sqrt[3]{2})] = 2$$
Basis for $\mathbb{Q}(a)$ over $\mathbb{Q}(\sqrt[3]{2})$ is $\{1, a\}$.
Thus basis for $\mathbb{Q}(a)$ over $\mathbb{Q}$ is the products:
$$\{1, 2^{1/3}, 2^{2/3}, a, 2^{1/3}a, 2^{2/3}a \}$$

## Q4

$$a = \sqrt{2} + \sqrt[3]{4}$$
$$(a - \sqrt[3]{4})^2 = 2$$
$$a^2 - 2 \sqrt[3]{4} + 4^{2/3} - 2 = 0$$
$$a^2 = 2 + 2 \cdot 4^{1/3} - 4^{2/3}$$
$$a^2 \in \mathbb{Q}(\sqrt{2} + \sqrt[3]{4}) \implies 4^{1/3} \in \mathbb{Q}(\sqrt{2} + \sqrt[3]{4})$$
$$x = \sqrt[3]{4}$$
$$\therefore x^3 - 4 = 0$$
$$[\mathbb{Q}(4^{\frac{1}{3}}): \mathbb{Q}] = 3$$
Basis is $\{1, 4^{\frac{1}{3}}, 4^{\frac{2}{3}}\}$.
From earlier $a^2 = 2 + 2 \cdot 4^{\frac{1}{3}} - 4^{\frac{2}{3}}$ so $[\mathbb{Q}(\sqrt{2} + \sqrt[3]{4}):\mathbb{Q}(4^{\frac{1}{3}})] = 2$.

Note that $4^{\frac{1}{3}} \notin \mathbb{Q}(2^{\frac{1}{2}})$, otherwise $4^{1/3} = a + b2^{\frac{1}{2}}$ which is impossible, since squaring both sides would lead to a contradiction. So $\mathbb{Q}(2^{\frac{1}{2}}) = \mathbb{Q}(2^{\frac{1}{2}}, 4^{\frac{1}{3}})$/

Basis for $\mathbb{Q}(2^{\frac{1}{2}} + 4^{\frac{1}{3}})$

$$\{1, 4^{\frac{1}{3}}, 4^{\frac{2}{3}}, 2^{\frac{1}{2}}, 4^{\frac{1}{3}}2^{\frac{1}{2}}, 4^{\frac{2}{3}}2^{\frac{1}{2}}\}$$

